Refactor, tidy and doc ProcessOperations.s.dfy

src/dafny/beacon/statetransition/ProcessOperations.s.dfy
@@ -30,7 +30,7 @@ include "ProcessOperations.p.dfy"
 
 
 /**
- *  Proofs for process operations
+ * Process operations functional specification.
  */
 module ProcessOperationsSpec {
     
@@ -50,44 +50,86 @@ module ProcessOperationsSpec {
     import opened SSZ
     import opened ProcessOperationsProofs
 
+    //  Specifications of predicates and functions related to the process operation methods.
+    //  e.g. process_proposer_slashing, process_deposit, etc
+    //  For each process operations method there is a corresponding functional equivalent,
+    //  as well as another functional representation of the processing of a sequence of such values.
+    //  e.g. process_proposer_slashing --> updateProposerSlashing and updateProposerSlashings.
+    //  The predicates are used to represent preconditions for the various components.
+
+    // Predicates
+
+    /**
+     *  Check preconditions for a sequence of proposer slashings.
+     *  
+     *  @param  s       A beacon state.
+     *  @param  bb      A beacon block body. 
+     *  @returns        True if all bb.proposer_slashings[i] satisfy the preconditions
+     *                  of process_proposer_slashing & updateProposerSlashings.
+     */
     predicate isValidProposerSlashings(s: BeaconState, bb: BeaconBlockBody)
         requires minimumActiveValidators(s)
         requires  |s.validators| == |s.balances|
     {
         // proposer slashing preconditions
-        (forall i,j :: 0 <= i < j < |bb.proposer_slashings| && i != j ==> bb.proposer_slashings[i].header_1.proposer_index!= bb.proposer_slashings[j].header_1.proposer_index) // ve indices are unique
+        (forall i,j :: 0 <= i < j < |bb.proposer_slashings| && i != j 
+            ==> bb.proposer_slashings[i].header_1.proposer_index 
+                != bb.proposer_slashings[j].header_1.proposer_index) // ve indices are unique
         &&
         (forall i :: 0 <= i < |bb.proposer_slashings| ==> 
             bb.proposer_slashings[i].header_1.slot == bb.proposer_slashings[i].header_2.slot
-            && bb.proposer_slashings[i].header_1.proposer_index == bb.proposer_slashings[i].header_2.proposer_index
+            && bb.proposer_slashings[i].header_1.proposer_index 
+                == bb.proposer_slashings[i].header_2.proposer_index
             && bb.proposer_slashings[i].header_1 == bb.proposer_slashings[i].header_2
             && bb.proposer_slashings[i].header_1.proposer_index as int < |s.validators| 
             && !s.validators[bb.proposer_slashings[i].header_1.proposer_index].slashed 
-            && s.validators[bb.proposer_slashings[i].header_1.proposer_index].activation_epoch <= get_current_epoch(s) < s.validators[bb.proposer_slashings[i].header_1.proposer_index].withdrawable_epoch)
+            && s.validators[bb.proposer_slashings[i].header_1.proposer_index].activation_epoch 
+                <= get_current_epoch(s) 
+                < s.validators[bb.proposer_slashings[i].header_1.proposer_index].withdrawable_epoch)
     }
 
+    /**
+     *  Check preconditions for a sequence of attester slashings.
+     *  
+     *  @param  s       A beacon state.
+     *  @param  bb      A beacon block body. 
+     *  @returns        True if all bb.attester_slashings[i] satisfy the preconditions
+     *                  of process_attester_slashing & updateAttesterSlashings.
+     */
     predicate isValidAttesterSlashings(s: BeaconState, bb: BeaconBlockBody)
         requires minimumActiveValidators(s)
         requires  |s.validators| == |s.balances|
     {
         // attester slashing preconditions
         (forall i :: 0 <= i < |bb.attester_slashings| ==> 
-            forall j :: 0 <= j < |bb.attester_slashings[i].attestation_1.attesting_indices| ==> bb.attester_slashings[i].attestation_1.attesting_indices[j] as int < |s.validators| )
+            forall j :: 0 <= j < |bb.attester_slashings[i].attestation_1.attesting_indices| 
+                ==> bb.attester_slashings[i].attestation_1.attesting_indices[j] as int < |s.validators| )
 
         && (forall i :: 0 <= i < |bb.attester_slashings| ==> 
-            forall j :: 0 <= j < |bb.attester_slashings[i].attestation_2.attesting_indices| ==> bb.attester_slashings[i].attestation_2.attesting_indices[j] as int < |s.validators|)
+            forall j :: 0 <= j < |bb.attester_slashings[i].attestation_2.attesting_indices| 
+                ==> bb.attester_slashings[i].attestation_2.attesting_indices[j] as int < |s.validators|)
             
         && (forall i :: 0 <= i < |bb.attester_slashings| ==> 
-            && is_valid_indexed_attestation(s, bb.attester_slashings[i].attestation_1)
-            && is_valid_indexed_attestation(s, bb.attester_slashings[i].attestation_2)
-            && |sorted_intersection(bb.attester_slashings[i].attestation_1.attesting_indices, bb.attester_slashings[i].attestation_2.attesting_indices)| > 0
-            && is_slashable_attestation_data(bb.attester_slashings[i].attestation_1.data, bb.attester_slashings[i].attestation_2.data)
-            && is_valid_indexed_attestation(s, bb.attester_slashings[i].attestation_1)
-            && is_valid_indexed_attestation(s, bb.attester_slashings[i].attestation_2)
-            && |sorted_intersection(bb.attester_slashings[i].attestation_1.attesting_indices, bb.attester_slashings[i].attestation_2.attesting_indices)| > 0
+            var a1 := bb.attester_slashings[i].attestation_1;
+            var a2 := bb.attester_slashings[i].attestation_2;
+            && is_valid_indexed_attestation(s, a1)
+            && is_valid_indexed_attestation(s, a2)
+            && |sorted_intersection(a1.attesting_indices, a2.attesting_indices)| > 0
+            && is_slashable_attestation_data(a1.data, a2.data)
+            && is_valid_indexed_attestation(s, a1)
+            && is_valid_indexed_attestation(s, a2)
+            && |sorted_intersection(a1.attesting_indices, a2.attesting_indices)| > 0
         )
     }
 
+    /**
+     *  Check preconditions for a sequence of attestations.
+     *  
+     *  @param  s       A beacon state.
+     *  @param  bb      A beacon block body. 
+     *  @returns        True if all bb.attestations[i] satisfy the preconditions
+     *                  of process_attestation & updateAttestations.
+     */
     predicate isValidAttestations(s: BeaconState, bb: BeaconBlockBody)
         requires minimumActiveValidators(s)
         requires  |s.validators| == |s.balances|
@@ -95,10 +137,20 @@ module ProcessOperationsSpec {
         // process attestation preconditions
         |bb.attestations| as nat <= MAX_ATTESTATIONS as nat
         && (forall i:: 0 <= i < |bb.attestations| ==> attestationIsWellFormed(s, bb.attestations[i]))
-        && |s.current_epoch_attestations| as nat + |bb.attestations| as nat <= MAX_ATTESTATIONS as nat * SLOTS_PER_EPOCH as nat 
-        && |s.previous_epoch_attestations| as nat + |bb.attestations| as nat <= MAX_ATTESTATIONS as nat * SLOTS_PER_EPOCH as nat 
+        && |s.current_epoch_attestations| as nat + |bb.attestations| as nat 
+            <= MAX_ATTESTATIONS as nat * SLOTS_PER_EPOCH as nat 
+        && |s.previous_epoch_attestations| as nat + |bb.attestations| as nat 
+            <= MAX_ATTESTATIONS as nat * SLOTS_PER_EPOCH as nat 
     }
 
+    /**
+     *  Check preconditions for a sequence of deposits.
+     *  
+     *  @param  s       A beacon state.
+     *  @param  bb      A beacon block body. 
+     *  @returns        True if bb.deposits satisfies the preconditions of process_deposit
+     *                  & updateDeposits.
+     */
     predicate isValidDeposits(s: BeaconState, bb: BeaconBlockBody)
         requires minimumActiveValidators(s)
         requires  |s.validators| == |s.balances|
@@ -109,41 +161,100 @@ module ProcessOperationsSpec {
         && (total_balances(s.balances) + total_deposits(bb.deposits) < 0x10000000000000000 )
     }
 
+    /**
+     *  Check preconditions for a sequence of voluntary exits.
+     *  
+     *  @param  s       A beacon state.
+     *  @param  bb      A beacon block body. 
+     *  @returns        True if all bb.voluntary_exits[i] satisfy the preconditions
+     *                  of process_voluntary_exit & updateVoluntaryExits.
+     */
     predicate isValidVoluntaryExits(s: BeaconState, bb: BeaconBlockBody)
         requires minimumActiveValidators(s)
         requires  |s.validators| == |s.balances|
     {
         // voluntary exit preconditions
-        (forall i,j :: 0 <= i < j < |bb.voluntary_exits| && i != j ==> bb.voluntary_exits[i].validator_index != bb.voluntary_exits[j].validator_index )// ve indices are unique
+        // indices are unique
+        (forall i,j :: 0 <= i < j < |bb.voluntary_exits| && i != j 
+            ==> bb.voluntary_exits[i].validator_index != bb.voluntary_exits[j].validator_index )
+        
         && (forall i :: 0 <= i < |bb.voluntary_exits| ==> 
              bb.voluntary_exits[i].validator_index as int < |s.validators| 
              && get_current_epoch(s) >= bb.voluntary_exits[i].epoch
              && !s.validators[bb.voluntary_exits[i].validator_index].slashed
-             && s.validators[bb.voluntary_exits[i].validator_index].activation_epoch <= get_current_epoch(s) < s.validators[bb.voluntary_exits[i].validator_index].withdrawable_epoch
+             && s.validators[bb.voluntary_exits[i].validator_index].activation_epoch 
+                <= get_current_epoch(s) 
+                < s.validators[bb.voluntary_exits[i].validator_index].withdrawable_epoch
              && s.validators[bb.voluntary_exits[i].validator_index].exitEpoch == FAR_FUTURE_EPOCH
-             && (get_current_epoch(s) as nat >= s.validators[bb.voluntary_exits[i].validator_index].activation_epoch as nat + SHARD_COMMITTEE_PERIOD as nat)
+             && (get_current_epoch(s) as nat 
+                >= s.validators[bb.voluntary_exits[i].validator_index].activation_epoch as nat 
+                    + SHARD_COMMITTEE_PERIOD as nat)
             )
     }
 
+    /**
+     *  Check preconditions required for a beacon block body to be processed.
+     *  
+     *  @param  s       A beacon state.
+     *  @param  bb      A beacon block body. 
+     *  @returns        True if all bb satisfies the preconditions of process_operations/updateOperations.
+     *     
+     *  @notes          A proof could be constructed to show that the intermediate states apply a s.
+     *                  i.e. simplify to remove updateAttesterSlashings, updateAttestations, etc.
+     */
     predicate isValidBeaconBlockBody(s: BeaconState, bb: BeaconBlockBody)
         requires minimumActiveValidators(s)
         requires  |s.validators| == |s.balances|
-        // Note: A proof could be constructed to show that the intermediate states apply for s as well.
-        //      i.e. try to show the preconditions based on state s
     {
         isValidProposerSlashings(s, bb)
         && isValidAttesterSlashings(updateProposerSlashings(s, bb.proposer_slashings), bb)
-        && isValidAttestations(updateAttesterSlashings(updateProposerSlashings(s, bb.proposer_slashings), bb.attester_slashings), bb)
-        && isValidDeposits(updateAttestations(updateAttesterSlashings(updateProposerSlashings(s, bb.proposer_slashings), bb.attester_slashings), bb.attestations),bb)
-        && isValidVoluntaryExits(updateDeposits(updateAttestations(updateAttesterSlashings(updateProposerSlashings(s, bb.proposer_slashings), bb.attester_slashings), bb.attestations),bb.deposits),bb)
+        && isValidAttestations(
+                updateAttesterSlashings(
+                    updateProposerSlashings(s, bb.proposer_slashings), 
+                    bb.attester_slashings), 
+                bb)
+        && isValidDeposits(
+                updateAttestations(
+                    updateAttesterSlashings(
+                        updateProposerSlashings(s, bb.proposer_slashings), 
+                        bb.attester_slashings), 
+                    bb.attestations),
+                bb)
+        && isValidVoluntaryExits(
+                updateDeposits(
+                    updateAttestations(
+                        updateAttesterSlashings(
+                            updateProposerSlashings(s, bb.proposer_slashings), 
+                            bb.attester_slashings), 
+                        bb.attestations),
+                    bb.deposits),
+                bb)
     }
 
+
+    // Functional equivalents
+
+    /**
+     *  The functional equivalent of process_operations.
+     *  
+     *  @param  s       A beacon state.
+     *  @param  bb      A beacon block body. 
+     *  @returns        A new state obtained from processing operations.        
+     */
     function updateOperations(s: BeaconState, bb: BeaconBlockBody): BeaconState
         requires  |s.validators| == |s.balances|
         requires |get_active_validator_indices(s.validators, get_current_epoch(s))| > 0
         requires isValidBeaconBlockBody(s, bb)
 
-        ensures updateOperations(s, bb) == updateVoluntaryExits(updateDeposits(updateAttestations(updateAttesterSlashings(updateProposerSlashings(s, bb.proposer_slashings), bb.attester_slashings), bb.attestations), bb.deposits), bb.voluntary_exits)
+        ensures updateOperations(s, bb) == updateVoluntaryExits(
+                                            updateDeposits(
+                                                updateAttestations(
+                                                    updateAttesterSlashings(
+                                                        updateProposerSlashings(s, bb.proposer_slashings), 
+                                                        bb.attester_slashings), 
+                                                    bb.attestations), 
+                                                bb.deposits), 
+                                            bb.voluntary_exits)
     {
         //assert isValidProposerSlashings(s, bb);
         var s1 := updateProposerSlashings(s, bb.proposer_slashings);
@@ -151,651 +262,49 @@ module ProcessOperationsSpec {
         //assert get_current_epoch(s1) == get_current_epoch(s);
         
         var s2 := updateAttesterSlashings(s1, bb.attester_slashings);
-        assert s2 == updateAttesterSlashings(updateProposerSlashings(s, bb.proposer_slashings), bb.attester_slashings);
+        assert s2 == updateAttesterSlashings(
+                        updateProposerSlashings(s, bb.proposer_slashings), 
+                        bb.attester_slashings);
         
         var s3 := updateAttestations(s2, bb.attestations);
-        assert s3 == updateAttestations(updateAttesterSlashings(updateProposerSlashings(s, bb.proposer_slashings), bb.attester_slashings), bb.attestations);
+        assert s3 == updateAttestations(
+                        updateAttesterSlashings(
+                            updateProposerSlashings(s, bb.proposer_slashings), 
+                            bb.attester_slashings), 
+                        bb.attestations);
         
         var s4 := updateDeposits(s3, bb.deposits);
-        assert s4 == updateDeposits(updateAttestations(updateAttesterSlashings(updateProposerSlashings(s, bb.proposer_slashings), bb.attester_slashings), bb.attestations), bb.deposits);
+        assert s4 == updateDeposits(
+                        updateAttestations(
+                            updateAttesterSlashings(
+                                updateProposerSlashings(s, bb.proposer_slashings), 
+                                bb.attester_slashings), 
+                            bb.attestations), 
+                        bb.deposits);
 
-         var s5 := updateVoluntaryExits(s4, bb.voluntary_exits);
-        assert s5 == updateVoluntaryExits(updateDeposits(updateAttestations(updateAttesterSlashings(updateProposerSlashings(s, bb.proposer_slashings), bb.attester_slashings), bb.attestations), bb.deposits), bb.voluntary_exits);
+        var s5 := updateVoluntaryExits(s4, bb.voluntary_exits);
+        assert s5 == updateVoluntaryExits(
+                        updateDeposits(
+                            updateAttestations(
+                                updateAttesterSlashings(
+                                    updateProposerSlashings(s, bb.proposer_slashings), 
+                                    bb.attester_slashings), 
+                                bb.attestations), 
+                            bb.deposits), 
+                        bb.voluntary_exits);
         
         s5
     }
 
-    
     /**
-     *  Take into account deposits in a block.
-     *
-     *  @param  s           A beacon state.
-     *  @param  deposits    A list of deposits from a block body.
-     *  @returns            The state obtained after taking account the deposits in `body` from state `s` 
-     */
-    function updateDeposits(s: BeaconState, deposits: seq<Deposit>) : BeaconState 
-        requires minimumActiveValidators(s)
-        requires s.eth1_deposit_index as int +  |deposits| < 0x10000000000000000 
-        requires |s.validators| == |s.balances|
-        requires |s.validators| + |deposits| <= VALIDATOR_REGISTRY_LIMIT as int
-        //requires forall i,j :: 0 <= i < j < |s.validators| ==> s.validators[i].pubkey != s.validators[j].pubkey
-
-        requires total_balances(s.balances) + total_deposits(deposits) < 0x10000000000000000 // less than total eth
-        //requires forall i :: 0 <= i < |s.validators| ==> s.balances[i] as int + get_deposit_total(s.validators[i].pubkey, deposits) as int < 0x10000000000000000
-        
-        //ensures updateDeposits(s, deposits).slot == s.slot 
-        //ensures updateDeposits(s, deposits).latest_block_header == s.latest_block_header
-        //ensures updateDeposits(s, deposits).block_roots == s.block_roots
-        //ensures updateDeposits(s, deposits).state_roots == s.state_roots
-
-        ensures updateDeposits(s, deposits).eth1_deposit_index == s.eth1_deposit_index  + |deposits| as uint64 
-        ensures |s.validators| <= |updateDeposits(s,deposits).validators| <= |s.validators| + |deposits| 
-        
-        // include properties ???
-        //ensures |updateDeposits(s,deposits).validators| == |updateDeposits(s,deposits).balances|        
-        //ensures |s.balances| <= |updateDeposits(s,deposits).balances| <= |s.balances| + |deposits| 
-
-        ensures total_balances(updateDeposits(s,deposits).balances) == total_balances(s.balances) + total_deposits(deposits)
-        ensures get_current_epoch(updateDeposits(s, deposits)) == get_current_epoch(s)
-        ensures minimumActiveValidators(updateDeposits(s, deposits))
-        
-         decreases |deposits|
-    {
-        if |deposits| == 0 then s
-        else 
-            //assert |deposits| > 0;
-            //assert forall i :: 0 <= i < |s.validators| ==> s.balances[i] as int + get_deposit_total(s.validators[i].pubkey, deposits) as int < 0x10000000000000000
-            //assert total_balances(s.balances) + total_deposits(deposits[..|deposits|-1]) < 0x10000000000000000 ;
-            //assert total_deposits(deposits[..|deposits|-1]) + total_deposits([deposits[|deposits|-1]]) == total_deposits(deposits) ;
-            //updateDeposits(s,deposits[..|deposits|-1])
-            //assert total_balances(s.balances) + total_deposits([deposits[|deposits|-1]]) < 0x10000000000000000;
-            //updateBalancesLemma(s,deposits);
-            //assert total_balances(s.balances) + total_deposits(deposits[..|deposits|-1]) < 0x10000000000000000;
-            //assert deposits[|deposits|-1].data.amount as int < total_deposits(deposits);
-            //assert total_balances(updateDeposits(s,deposits[..|deposits|-1]).balances) + deposits[|deposits|-1].data.amount as int < 0x10000000000000000;
-
-            //updateBalTotalBySingleDeposit(updateDeposits(s,deposits[..|deposits|-1]), deposits[|deposits|-1]);
-
-            updateDeposit(updateDeposits(s,deposits[..|deposits|-1]),deposits[|deposits|-1])
-    }
-
-    /**
-     *  Take into account a single deposit from a block.
-     *
+     *  The functional equivalent of process_proposer_slashing.
+     *  
      *  @param  s       A beacon state.
-     *  @param  d       A single deposit.
-     *  @returns        The state obtained after taking account the deposit `d` from state `s` 
+     *  @param  ps      A proposer slashing. 
+     *  @returns        A new state obtained from processing a proposer slashing.        
      */
-    function updateDeposit(s: BeaconState, d: Deposit) : BeaconState 
-        requires s.eth1_deposit_index as int +  1 < 0x10000000000000000 
-        requires |s.validators| == |s.balances|
-        requires |s.validators| + 1 <= VALIDATOR_REGISTRY_LIMIT as int
-        requires total_balances(s.balances) + d.data.amount as int < 0x10000000000000000
-        
-        //requires d.data.pubkey in seqKeysInValidators(s.validators) ==> s.balances[get_validator_index(seqKeysInValidators(s.validators), d.data.pubkey)] as int + d.data.amount as int < 0x10000000000000000
-        
-        ensures d.data.pubkey !in seqKeysInValidators(s.validators) ==> updateDeposit(s,d).validators == s.validators + [get_validator_from_deposit(d)]
-        ensures d.data.pubkey in seqKeysInValidators(s.validators)  ==> updateDeposit(s,d).validators == s.validators 
-        
-        ensures updateDeposit(s,d).eth1_deposit_index == s.eth1_deposit_index + 1
-        //ensures updateDeposit(s,d).slot == s.slot
-        //ensures updateDeposit(s,d).latest_block_header == s.latest_block_header
-        //ensures updateDeposit(s,d).block_roots == s.block_roots
-        //ensures updateDeposit(s,d).state_roots == s.state_roots
-
-        ensures |updateDeposit(s,d).validators| == |updateDeposit(s,d).balances|        // maybe include in property lemmas
-        ensures |s.validators| <= |updateDeposit(s,d).validators| <= |s.validators| + 1 // maybe include in property lemmas
-        ensures |s.balances| <= |updateDeposit(s,d).balances| <= |s.balances| + 1 // maybe include in property lemmas
-        ensures forall i :: 0 <= i < |s.balances| ==> s.balances[i] <= updateDeposit(s,d).balances[i]
-        //ensures total_balances(updateDeposit(s,d).balances) == total_balances(s.balances) + d.data.amount as int < 0x10000000000000000
-        // in lemma
-
-        ensures total_balances(updateDeposit(s,d).balances) == total_balances(s.balances) + d.data.amount as int < 0x10000000000000000
-        
-    {
-        var pk := seqKeysInValidators(s.validators); 
-        
-        s.(
-            eth1_deposit_index := (s.eth1_deposit_index as int + 1) as uint64,
-            validators := if d.data.pubkey in pk then 
-                                s.validators // unchanged validator members
-                            else 
-                                validator_append(s.validators, get_validator_from_deposit(d)), //(s.validators + [get_validator_from_deposit(d)]),
-            balances := if d.data.pubkey in pk then 
-                                individualBalanceBoundMaintained(s.balances,d);
-                                //assert s.balances[get_validator_index(pk, d.data.pubkey)] as int + d.data.amount as int < 0x10000000000000000;
-                                updateExistingBalance(s, get_validator_index(pk, d.data.pubkey), d.data.amount);
-                                increase_balance(s,get_validator_index(pk, d.data.pubkey),d.data.amount).balances
-                            else 
-                                distBalancesProp(s.balances,[d.data.amount]);
-                                balance_append(s.balances, d.data.amount) //s.balances + [d.data.amount]
-        )
-
-        //assert total_balances(s1.balances) == total_balances(s.balances) + d.data.amount as int < 0x10000000000000000;
-        //s1
-    }
-
-
-
-    
-
-   
-
-    function updateAttestation(s: BeaconState, a: Attestation) : BeaconState
-        requires attestationIsWellFormed(s, a)
-        requires |s.current_epoch_attestations| < MAX_ATTESTATIONS as nat * SLOTS_PER_EPOCH as nat 
-        requires |s.previous_epoch_attestations| < MAX_ATTESTATIONS as nat * SLOTS_PER_EPOCH as nat 
-        requires minimumActiveValidators(s)
-        ensures minimumActiveValidators(updateAttestation(s, a))
-        ensures |updateAttestation(s, a).current_epoch_attestations| + |updateAttestation(s, a).previous_epoch_attestations| ==
-                |s.current_epoch_attestations| + |s.previous_epoch_attestations| + 1
-        ensures |s.current_epoch_attestations| <= |updateAttestation(s, a).current_epoch_attestations| <= |s.current_epoch_attestations| + 1
-        ensures |s.previous_epoch_attestations| <=|updateAttestation(s, a).previous_epoch_attestations| <= |s.previous_epoch_attestations| + 1
-
-        ensures updateAttestation(s, a) == s.(current_epoch_attestations := updateAttestation(s, a).current_epoch_attestations) ||
-                 updateAttestation(s, a) == s.(previous_epoch_attestations := updateAttestation(s, a).previous_epoch_attestations)
-        ensures updateAttestation(s, a).validators == s.validators
-        ensures updateAttestation(s, a).balances == s.balances
-        ensures updateAttestation(s, a).slot == s.slot
-        ensures updateAttestation(s, a).current_justified_checkpoint == s.current_justified_checkpoint
-        ensures updateAttestation(s, a).previous_justified_checkpoint == s.previous_justified_checkpoint
-        ensures updateAttestation(s, a).eth1_deposit_index == s.eth1_deposit_index
-
-    {
-        // data = attestation.data
-        assert get_previous_epoch(s) <= a.data.target.epoch <=  get_current_epoch(s);
-        assert a.data.target.epoch == compute_epoch_at_slot(a.data.slot);
-        assert a.data.slot as nat + MIN_ATTESTATION_INCLUSION_DELAY as nat <= s.slot as nat <= a.data.slot as nat + SLOTS_PER_EPOCH as nat;
-        assert a.data.index < get_committee_count_per_slot(s, a.data.target.epoch);
-
-        var committee := get_beacon_committee(s, a.data.slot, a.data.index);
-        assert |a.aggregation_bits| == |committee|;
-
-        var pending_attestation := PendingAttestation(
-            a.aggregation_bits, 
-            a.data, 
-            (s.slot - a.data.slot), 
-            get_beacon_proposer_index(s) 
-        );
-
-        if a.data.target.epoch == get_current_epoch(s) then
-            //  Add a to current attestations
-            assert a.data.source == s.current_justified_checkpoint;
-            s.(
-                current_epoch_attestations := s.current_epoch_attestations + [pending_attestation]
-            )
-            // s.current_epoch_attestations.append(pending_attestation)
-        
-        else 
-            assert a.data.source == s.previous_justified_checkpoint;
-            s.(
-                previous_epoch_attestations := s.previous_epoch_attestations + [pending_attestation]
-            )
-        
-            // s.previous_epoch_attestations.append(pending_attestation)
-            
-        // # Verify signature
-        // Not implemented as part of the simplificiation
-        //assert is_valid_indexed_attestation(s', get_indexed_attestation(s', a));
-    }
-
-    function updateAttestations(s: BeaconState, a: seq<Attestation>) : BeaconState
-        requires |s.validators| == |s.balances|
-        requires |a| as nat <= MAX_ATTESTATIONS as nat
-        requires forall i:: 0 <= i < |a| ==> attestationIsWellFormed(s, a[i])
-        requires |s.current_epoch_attestations| as nat + |a| as nat <= MAX_ATTESTATIONS as nat * SLOTS_PER_EPOCH as nat 
-        requires |s.previous_epoch_attestations| as nat + |a| as nat <= MAX_ATTESTATIONS as nat * SLOTS_PER_EPOCH as nat 
-        requires minimumActiveValidators(s)
-        
-        ensures |updateAttestations(s,a).validators| == |updateAttestations(s,a).balances|
-        ensures |updateAttestations(s,a).current_epoch_attestations| + |updateAttestations(s,a).previous_epoch_attestations| ==
-                |s.current_epoch_attestations| + |s.previous_epoch_attestations| + |a|
-        ensures |updateAttestations(s,a).current_epoch_attestations| <= |s.current_epoch_attestations| + |a|;
-        ensures |updateAttestations(s,a).previous_epoch_attestations| <= |s.previous_epoch_attestations| + |a|;
-
-        ensures minimumActiveValidators(updateAttestations(s, a))
-        ensures updateAttestations(s, a).validators == s.validators
-        ensures updateAttestations(s, a).slot == s.slot
-        ensures updateAttestations(s, a).current_justified_checkpoint == s.current_justified_checkpoint
-        ensures updateAttestations(s, a).previous_justified_checkpoint == s.previous_justified_checkpoint
-        // could add an ensures to demonstrate the fields changed i.e. current_epoch_attestations etc
-        ensures updateAttestations(s, a).eth1_deposit_index == s.eth1_deposit_index
-    {
-        if |a| == 0 then s
-        else 
-
-            // data = attestation.data
-            var index := |a| -1;
-            // these should allow follow from the original preconditions
-            // assert |a[..index]| as nat <= MAX_ATTESTATIONS as nat;
-            // assert forall i:: 0 <= i < |a[..index]| ==> attestationIsWellFormed(s, a[i]);
-            // assert |s.current_epoch_attestations| as nat + |a[..index]| as nat <= MAX_ATTESTATIONS as nat * SLOTS_PER_EPOCH as nat ;
-            // assert |s.previous_epoch_attestations| as nat + |a[..index]| as nat <= MAX_ATTESTATIONS as nat * SLOTS_PER_EPOCH as nat ;
-            // assert minimumActiveValidators(s);
-
-            var s1 := updateAttestations(s,a[..index]);
-
-            // these relate to the nested state == updateAttestations(s,a[..index])
-            // assert s1.validators == s.validators;
-            // assert s1.slot == s.slot;
-            // assert s1.current_justified_checkpoint == s.current_justified_checkpoint;
-            // assert s1.previous_justified_checkpoint == s.previous_justified_checkpoint;
-            AttestationHelperLemma(s, s1, a[index]);
-
-            //assert attestationIsWellFormed(s1, a[index]);
-
-            assert |s1.current_epoch_attestations| + |s1.previous_epoch_attestations| ==
-                |s.current_epoch_attestations| + |s.previous_epoch_attestations| + |a[..index]|;
-            assert |s1.current_epoch_attestations| <= |s.current_epoch_attestations| + |a[..index]|;
-            assert |s1.previous_epoch_attestations| <= |s.previous_epoch_attestations| + |a[..index]|;
-
-            assert |a[..index]| < |a|;
-            assert |updateAttestations(s,a[..index]).current_epoch_attestations| < MAX_ATTESTATIONS as nat * SLOTS_PER_EPOCH as nat ;
-            assert |updateAttestations(s,a[..index]).previous_epoch_attestations| < MAX_ATTESTATIONS as nat * SLOTS_PER_EPOCH as nat ;
-            assert minimumActiveValidators(updateAttestations(s,a[..index]));
-
-            updateAttestation(s1, a[index])
-    }
-
-    // function updateVoluntaryExit(s: BeaconState, voluntary_exit: VoluntaryExit) : BeaconState
-    //     requires |s.validators| == |s.balances|
-    //     requires voluntary_exit.validator_index as int < |s.validators| 
-    //     //requires minimumActiveValidators(s)
-    //     // requires is_active_validator(s.validators[voluntary_exit.validator_index], get_current_epoch(s))
-    //     // (!v.slashed) && (v.activation_epoch <= epoch < v.withdrawable_epoch)
-    //     requires !s.validators[voluntary_exit.validator_index].slashed
-    //     requires s.validators[voluntary_exit.validator_index].activation_epoch <= get_current_epoch(s) < s.validators[voluntary_exit.validator_index].withdrawable_epoch
-
-    //     requires s.validators[voluntary_exit.validator_index].exitEpoch == FAR_FUTURE_EPOCH
-    //     requires get_current_epoch(s) >= voluntary_exit.epoch
-    //     requires get_current_epoch(s) >= s.validators[voluntary_exit.validator_index].activation_epoch + SHARD_COMMITTEE_PERIOD 
-        
-    //     // the next requires is to prevent overflow
-    //     //requires max_epoch(get_exit_epochs(s.validators) + [compute_activation_exit_epoch(get_current_epoch(s))]) as int + 1 + MIN_VALIDATOR_WITHDRAWABILITY_DELAY < 0x10000000000000000
-        
-    //     ensures |updateVoluntaryExit(s, voluntary_exit).validators| == |s.validators| 
-    //     ensures |updateVoluntaryExit(s, voluntary_exit).validators| == |s.balances| 
-    //     ensures forall i :: 0 <= i < |s.validators| && i != voluntary_exit.validator_index as int ==> updateVoluntaryExit(s, voluntary_exit).validators[i] == s.validators[i]
-    //     //ensures forall i :: 0 <= i < |s.validators| && i != voluntary_exit.validator_index as int ==> updateVoluntaryExit(s, voluntary_exit).validators[i].exitEpoch == s.validators[i].exitEpoch
-        
-    //     ensures updateVoluntaryExit(s, voluntary_exit) == initiate_validator_exit(s, voluntary_exit.validator_index)
-    //     ensures get_current_epoch(updateVoluntaryExit(s, voluntary_exit)) == get_current_epoch(s)
-    //     ensures get_current_epoch(s) >= updateVoluntaryExit(s, voluntary_exit).validators[voluntary_exit.validator_index].activation_epoch + SHARD_COMMITTEE_PERIOD 
-    //     ensures forall i :: 0 <= i < |s.validators| ==> updateVoluntaryExit(s, voluntary_exit).validators[i].activation_epoch == s.validators[i].activation_epoch
-    //     ensures minimumActiveValidators(updateVoluntaryExit(s, voluntary_exit))
-    //     // ensures active validators haven't changed??
-    // {
-        
-    //     var exit_epochs := get_exit_epochs(s.validators);
-        
-    //     var exit_queue_epoch := max_epoch(exit_epochs + [compute_activation_exit_epoch(get_current_epoch(s))]);
-
-    //     assert compute_activation_exit_epoch(get_current_epoch(s)) > get_current_epoch(s);
-    //     assert compute_activation_exit_epoch(get_current_epoch(s)) in (exit_epochs + [compute_activation_exit_epoch(get_current_epoch(s))]);
-    //     assert max_epoch(exit_epochs + [compute_activation_exit_epoch(get_current_epoch(s))]) >= compute_activation_exit_epoch(get_current_epoch(s)); 
-    //     assert max_epoch(exit_epochs + [compute_activation_exit_epoch(get_current_epoch(s))]) > get_current_epoch(s);
-    //     assert exit_queue_epoch > get_current_epoch(s);
-
-    //     var exit_queue_churn := |get_queue_churn(s.validators, exit_queue_epoch)|;
-    //     var validator_churn_limit := get_validator_churn_limit(s);
-    //     var index := voluntary_exit.validator_index;
-        
-    //     assume exit_queue_epoch as int + 1 + MIN_VALIDATOR_WITHDRAWABILITY_DELAY as nat < 0x10000000000000000; 
-    //     assert minimumActiveValidators(s);
-    //     assert exists v :: 0 <= v < |s.validators| && s.validators[v].activation_epoch <= get_current_epoch(s) < s.validators[v].exitEpoch;
-        
-    //     var s1 := if exit_queue_churn  >= get_validator_churn_limit(s) as nat then 
-    //             s.(validators := s.validators[index as int := s.validators[index].(exitEpoch := exit_queue_epoch + 1 as Epoch,
-    //                                                                 withdrawable_epoch := (exit_queue_epoch as nat + 1 + MIN_VALIDATOR_WITHDRAWABILITY_DELAY as nat) as Epoch)])
-    //             else
-    //             s.(validators := s.validators[index as int := s.validators[index].(exitEpoch := exit_queue_epoch,
-    //                                                                 withdrawable_epoch := (exit_queue_epoch as nat + MIN_VALIDATOR_WITHDRAWABILITY_DELAY as nat) as Epoch)]);
-        
-    //     assert forall v :: 0 <= v < |s1.validators| ==>  s1.validators[v].activation_epoch ==  s.validators[v].activation_epoch;
-    //     assert forall v :: 0 <= v < |s1.validators| ==>  s1.validators[v].exitEpoch > get_current_epoch(s1) || s1.validators[v].exitEpoch == s1.validators[v].exitEpoch;
-    //     assert exists v :: 0 <= v < |s1.validators| && s1.validators[v].activation_epoch <= get_current_epoch(s1) < s1.validators[v].exitEpoch;
-    //     assert minimumActiveValidators(s1);
-    //     s1
-
-    // }
-
-    // function {:timeLimitMultiplier 1} updateVoluntaryExits(s: BeaconState, ve: seq<VoluntaryExit>) : BeaconState
-    //     requires minimumActiveValidators(s)
-    //     requires forall i,j :: 0 <= i < j < |ve| && i != j ==> ve[i].validator_index != ve[j].validator_index // ve indices are unique
-    //     requires |s.validators| == |s.balances|
-    //     requires forall i :: 0 <= i < |ve| ==> get_current_epoch(s) >= ve[i].epoch
-        
-    //     requires forall i :: 0 <= i < |ve| ==> ve[i].validator_index as int < |s.validators| 
-    //     //requires forall i :: 0 <= i < |ve| ==> is_active_validator(s.validators[ve[i].validator_index], get_current_epoch(s))
-    //     requires forall i :: 0 <= i < |ve| ==> !s.validators[ve[i].validator_index].slashed
-    //     requires forall i :: 0 <= i < |ve| ==> s.validators[ve[i].validator_index].activation_epoch <= get_current_epoch(s) < s.validators[ve[i].validator_index].withdrawable_epoch
-
-    //     requires forall i :: 0 <= i < |ve| ==> s.validators[ve[i].validator_index].exitEpoch == FAR_FUTURE_EPOCH
-    //     requires forall i :: 0 <= i < |ve| ==> s.validators[ve[i].validator_index].activation_epoch as nat + SHARD_COMMITTEE_PERIOD as nat <= get_current_epoch(s) as nat < 0x10000000000000000 
-
-    //     //requires forall i :: i in get_VolExit_validator_indices(ve) ==> 0 <= i < |s.validators| 
-        
-    //     // //requires forall i :: i in get_VolExit_validator_indices(ve) ==> is_active_validator(s.validators[i], get_current_epoch(s))
-    //     //requires forall i :: i in get_VolExit_validator_indices(ve) ==> !s.validators[i].slashed
-    //     //requires forall i :: i in get_VolExit_validator_indices(ve) ==> s.validators[i].activation_epoch <= get_current_epoch(s) < s.validators[i].withdrawable_epoch
-
-    //     //requires forall i :: i in get_VolExit_validator_indices(ve) ==> s.validators[i].exitEpoch == FAR_FUTURE_EPOCH
-    //     //requires forall i :: i in get_VolExit_validator_indices(ve) ==> get_current_epoch(s) >= s.validators[i].activation_epoch + SHARD_COMMITTEE_PERIOD 
-    
-    //     ensures |updateVoluntaryExits(s, ve).validators| == |s.validators|
-    //     ensures |updateVoluntaryExits(s, ve).validators| == |updateVoluntaryExits(s, ve).balances|
-    //     ensures updateVoluntaryExits(s, ve).slot == s.slot
-    //     ensures get_current_epoch(updateVoluntaryExits(s, ve)) == get_current_epoch(s)
-    //     ensures forall i :: 0 <= i < |s.validators| ==> updateVoluntaryExits(s, ve).validators[i].activation_epoch == s.validators[i].activation_epoch
-
-    //     ensures forall i :: 0 <= i < |s.validators| && i !in get_VolExit_validator_indices(ve) ==> updateVoluntaryExits(s, ve).validators[i] == s.validators[i]
-    //     ensures minimumActiveValidators(updateVoluntaryExits(s, ve))
-    //     //ensures forall i :: 0 <= i < |s.validators| && i !in get_VolExit_validator_indices(ve) ==> updateVoluntaryExits(s, ve).validators[i].exitEpoch == s.validators[i].exitEpoch
-    //     //ensures forall i :: 0 <= i < |s.validators| && i !in get_VolExit_validator_indices(ve) ==> updateVoluntaryExits(s, ve).validators[i].slashed == s.validators[i].slashed
-    //     //ensures forall i :: 0 <= i < |s.validators| && i !in get_VolExit_validator_indices(ve) ==> updateVoluntaryExits(s, ve).validators[i].withdrawable_epoch == s.validators[i].withdrawable_epoch
-    //     //ensures forall i :: 0 <= i < |s.validators| ==> forall j :: 0 <= j < |ve| && i != ve[j].validator_index as int ==> updateVoluntaryExits(s, ve).validators[i].exitEpoch == s.validators[i].exitEpoch
-
-    //     //ensures forall i :: 0 <= i < |ve| ==> get_current_epoch(s) >= updateVoluntaryExits(s, ve).validators[ve[i].validator_index].activation_epoch + SHARD_COMMITTEE_PERIOD
-    //     //ensures forall i :: 0 <= i < |ve| ==> is_active_validator(updateVoluntaryExits(s,ve).validators[ve[i].validator_index], get_current_epoch(s))
-    //     decreases |ve|
-    // {
-    //     if |ve| == 0 then 
-    //         //assert get_VolExit_validator_indices(ve) == [];
-    //         //assert forall i :: 0 <= i < |s.validators| && i !in get_VolExit_validator_indices(ve) ==> updateVoluntaryExits(s, ve).validators[i].exitEpoch == s.validators[i].exitEpoch;
-    //         s
-    //     // else if |ve| == 1 then
-    //     //     assert |ve[..|ve|-1]| == 0;
-    //     //     assert updateVoluntaryExits(s,ve[..|ve|-1]) == s;
-    //     //     assert forall i :: 0 <= i < |s.validators| && i !in get_VolExit_validator_indices(ve) ==> updateVoluntaryExits(s, ve).validators[i].exitEpoch == s.validators[i].exitEpoch;
-    //     //     updateVoluntaryExit(s, ve[|ve|-1])
-
-    //     else
-    //         helperVoluntaryExitLemma3(s, ve);
-    //         helperVoluntaryExitLemma2(s, ve);
-    //         assert forall i :: i in get_VolExit_validator_indices(ve[..|ve|-1]) ==> 0 <= i < |s.validators|; 
-
-    //         assert forall i :: i in get_VolExit_validator_indices(ve[..|ve|-1]) ==> !s.validators[i].slashed;
-    //         assert forall i :: i in get_VolExit_validator_indices(ve[..|ve|-1]) ==> s.validators[i].activation_epoch <= get_current_epoch(s) < s.validators[i].withdrawable_epoch;
-    //         assert forall i :: i in get_VolExit_validator_indices(ve[..|ve|-1]) ==> s.validators[i].exitEpoch == FAR_FUTURE_EPOCH;
-    //         assert forall i :: i in get_VolExit_validator_indices(ve[..|ve|-1]) ==> get_current_epoch(s) >= s.validators[i].activation_epoch + SHARD_COMMITTEE_PERIOD;
-    //         //assert forall i :: 0 <= i < |s.validators| && i !in get_VolExit_validator_indices(ve[..|ve|-1]) ==> 
-    //         //    updateVoluntaryExits(s,ve[..|ve|-1]).validators[i].exitEpoch == s.validators[i].exitEpoch;
-
-    //         // assert forall i :: 0 <= i < |s.validators| && i !in get_VolExit_validator_indices(ve[..|ve|-1]) ==> updateVoluntaryExits(s, ve[..|ve|-1]).validators[i].slashed == s.validators[i].slashed;
-    //         // assert ve[|ve|-1].validator_index as int !in get_VolExit_validator_indices(ve[..|ve|-1]) ==> 
-    //         //     updateVoluntaryExits(s, ve[..|ve|-1]).validators[ve[|ve|-1].validator_index].slashed  == s.validators[ve[|ve|-1].validator_index].slashed;
-    //         // assert !s.validators[ve[|ve|-1].validator_index].slashed;
-
-    //         // assert forall i :: 0 <= i < |s.validators| && i !in get_VolExit_validator_indices(ve[..|ve|-1]) ==> updateVoluntaryExits(s, ve[..|ve|-1]).validators[i].exitEpoch == s.validators[i].exitEpoch;
-    //         // assert ve[|ve|-1].validator_index as int !in get_VolExit_validator_indices(ve[..|ve|-1]) ==> 
-    //         //     updateVoluntaryExits(s, ve[..|ve|-1]).validators[ve[|ve|-1].validator_index].exitEpoch  == s.validators[ve[|ve|-1].validator_index].exitEpoch;
-    //         // assert ve[|ve|-1].validator_index as int in get_VolExit_validator_indices(ve) ==> s.validators[ve[|ve|-1].validator_index].exitEpoch == FAR_FUTURE_EPOCH;
-
-    //         assert |updateVoluntaryExits(s,ve[..|ve|-1]).validators| == |s.validators|;
-    //         mappingVolExitIndices(ve);
-    //         subsetMappingVolExitIndices(ve, |ve|-1);
-    //         //assume ve[|ve|-1].validator_index as int < |updateVoluntaryExits(s,ve[..|ve|-1]).validators|;
-    //         //assert forall i :: i in get_VolExit_validator_indices(ve) ==> i < |s.validators|;  // from requires
-    //         assert ve[|ve|-1].validator_index as int in get_VolExit_validator_indices(ve);
-
-    //         //assume get_current_epoch(updateVoluntaryExits(s,ve[..|ve|-1])) >= ve[|ve|-1].epoch;
-    //         assert get_current_epoch(updateVoluntaryExits(s,ve[..|ve|-1])) == get_current_epoch(s);
-    //         assert get_current_epoch(s) >= ve[|ve|-1].epoch; // from requires
-
-    //         helperVoluntaryExitLemma(updateVoluntaryExits(s,ve[..|ve|-1]), ve[|ve|-1]);
-    //         updateVoluntaryExit(updateVoluntaryExits(s,ve[..|ve|-1]), ve[|ve|-1])
-    // }
-
-
-    function updateVoluntaryExit(s: BeaconState, voluntary_exit: VoluntaryExit) : BeaconState
-        requires minimumActiveValidators(s)
-        requires |s.validators| == |s.balances|
-        requires voluntary_exit.validator_index as int < |s.validators| 
-        
-        requires !s.validators[voluntary_exit.validator_index].slashed
-        requires s.validators[voluntary_exit.validator_index].activation_epoch <= get_current_epoch(s) < s.validators[voluntary_exit.validator_index].withdrawable_epoch
-
-        requires s.validators[voluntary_exit.validator_index].exitEpoch == FAR_FUTURE_EPOCH
-        requires get_current_epoch(s) >= voluntary_exit.epoch
-        requires get_current_epoch(s) >= s.validators[voluntary_exit.validator_index].activation_epoch + SHARD_COMMITTEE_PERIOD 
-        
-        // the next requires is to prevent overflow
-        //requires max_epoch(get_exit_epochs(s.validators) + [compute_activation_exit_epoch(get_current_epoch(s))]) as int + 1 + MIN_VALIDATOR_WITHDRAWABILITY_DELAY < 0x10000000000000000
-        
-        ensures |updateVoluntaryExit(s, voluntary_exit).validators| == |s.validators| 
-        ensures |updateVoluntaryExit(s, voluntary_exit).validators| == |s.balances| 
-        ensures forall i :: 0 <= i < |s.validators| && i != voluntary_exit.validator_index as int ==> updateVoluntaryExit(s, voluntary_exit).validators[i] == s.validators[i]
-        //ensures forall i :: 0 <= i < |s.validators| && i != voluntary_exit.validator_index as int ==> updateVoluntaryExit(s, voluntary_exit).validators[i].exitEpoch == s.validators[i].exitEpoch
-        
-        ensures updateVoluntaryExit(s, voluntary_exit) == initiate_validator_exit(s, voluntary_exit.validator_index)
-        ensures get_current_epoch(updateVoluntaryExit(s, voluntary_exit)) == get_current_epoch(s)
-        ensures get_current_epoch(s) >= updateVoluntaryExit(s, voluntary_exit).validators[voluntary_exit.validator_index].activation_epoch + SHARD_COMMITTEE_PERIOD 
-        ensures forall i :: 0 <= i < |s.validators| ==> updateVoluntaryExit(s, voluntary_exit).validators[i].activation_epoch == s.validators[i].activation_epoch
-        ensures minimumActiveValidators(updateVoluntaryExit(s, voluntary_exit))
-        // ensures active validators haven't changed??
-    {
-        var s' := initiate_validator_exit(s, voluntary_exit.validator_index);
-        
-        assert minimumActiveValidators(s');
-        s'
-
-    }
-    
-    function {:timeLimitMultiplier 1} updateVoluntaryExits(s: BeaconState, ve: seq<VoluntaryExit>) : BeaconState
-        requires minimumActiveValidators(s)
-        requires forall i,j :: 0 <= i < j < |ve| && i != j ==> ve[i].validator_index != ve[j].validator_index // ve indices are unique
-        requires |s.validators| == |s.balances|
-        requires forall i :: 0 <= i < |ve| ==> get_current_epoch(s) >= ve[i].epoch
-        
-        requires forall i :: 0 <= i < |ve| ==> ve[i].validator_index as int < |s.validators| 
-        //requires forall i :: 0 <= i < |ve| ==> is_active_validator(s.validators[ve[i].validator_index], get_current_epoch(s))
-        requires forall i :: 0 <= i < |ve| ==> !s.validators[ve[i].validator_index].slashed
-        requires forall i :: 0 <= i < |ve| ==> s.validators[ve[i].validator_index].activation_epoch <= get_current_epoch(s) < s.validators[ve[i].validator_index].withdrawable_epoch
-
-        requires forall i :: 0 <= i < |ve| ==> s.validators[ve[i].validator_index].exitEpoch == FAR_FUTURE_EPOCH
-        requires forall i :: 0 <= i < |ve| ==> s.validators[ve[i].validator_index].activation_epoch as nat + SHARD_COMMITTEE_PERIOD as nat <= get_current_epoch(s) as nat < 0x10000000000000000 
-
-        //requires forall i :: i in get_VolExit_validator_indices(ve) ==> 0 <= i < |s.validators| 
-        
-        // //requires forall i :: i in get_VolExit_validator_indices(ve) ==> is_active_validator(s.validators[i], get_current_epoch(s))
-        //requires forall i :: i in get_VolExit_validator_indices(ve) ==> !s.validators[i].slashed
-        //requires forall i :: i in get_VolExit_validator_indices(ve) ==> s.validators[i].activation_epoch <= get_current_epoch(s) < s.validators[i].withdrawable_epoch
-
-        //requires forall i :: i in get_VolExit_validator_indices(ve) ==> s.validators[i].exitEpoch == FAR_FUTURE_EPOCH
-        //requires forall i :: i in get_VolExit_validator_indices(ve) ==> get_current_epoch(s) >= s.validators[i].activation_epoch + SHARD_COMMITTEE_PERIOD 
-    
-        ensures |updateVoluntaryExits(s, ve).validators| == |s.validators|
-        ensures |updateVoluntaryExits(s, ve).validators| == |updateVoluntaryExits(s, ve).balances|
-        ensures updateVoluntaryExits(s, ve).slot == s.slot
-        ensures get_current_epoch(updateVoluntaryExits(s, ve)) == get_current_epoch(s)
-        ensures forall i :: 0 <= i < |s.validators| ==> updateVoluntaryExits(s, ve).validators[i].activation_epoch == s.validators[i].activation_epoch
-
-        ensures forall i :: 0 <= i < |s.validators| && i !in get_VolExit_validator_indices(ve) ==> updateVoluntaryExits(s, ve).validators[i] == s.validators[i]
-        ensures minimumActiveValidators(updateVoluntaryExits(s, ve))
-        //ensures forall i :: 0 <= i < |s.validators| && i !in get_VolExit_validator_indices(ve) ==> updateVoluntaryExits(s, ve).validators[i].exitEpoch == s.validators[i].exitEpoch
-        //ensures forall i :: 0 <= i < |s.validators| && i !in get_VolExit_validator_indices(ve) ==> updateVoluntaryExits(s, ve).validators[i].slashed == s.validators[i].slashed
-        //ensures forall i :: 0 <= i < |s.validators| && i !in get_VolExit_validator_indices(ve) ==> updateVoluntaryExits(s, ve).validators[i].withdrawable_epoch == s.validators[i].withdrawable_epoch
-        //ensures forall i :: 0 <= i < |s.validators| ==> forall j :: 0 <= j < |ve| && i != ve[j].validator_index as int ==> updateVoluntaryExits(s, ve).validators[i].exitEpoch == s.validators[i].exitEpoch
-
-        //ensures forall i :: 0 <= i < |ve| ==> get_current_epoch(s) >= updateVoluntaryExits(s, ve).validators[ve[i].validator_index].activation_epoch + SHARD_COMMITTEE_PERIOD
-        //ensures forall i :: 0 <= i < |ve| ==> is_active_validator(updateVoluntaryExits(s,ve).validators[ve[i].validator_index], get_current_epoch(s))
-        decreases |ve|
-    {
-        if |ve| == 0 then 
-            //assert get_VolExit_validator_indices(ve) == [];
-            //assert forall i :: 0 <= i < |s.validators| && i !in get_VolExit_validator_indices(ve) ==> updateVoluntaryExits(s, ve).validators[i].exitEpoch == s.validators[i].exitEpoch;
-            s
-        // else if |ve| == 1 then
-        //     assert |ve[..|ve|-1]| == 0;
-        //     assert updateVoluntaryExits(s,ve[..|ve|-1]) == s;
-        //     assert forall i :: 0 <= i < |s.validators| && i !in get_VolExit_validator_indices(ve) ==> updateVoluntaryExits(s, ve).validators[i].exitEpoch == s.validators[i].exitEpoch;
-        //     updateVoluntaryExit(s, ve[|ve|-1])
-
-        else
-            helperVoluntaryExitLemma3(s, ve);
-            helperVoluntaryExitLemma2(s, ve);
-            assert forall i :: i in get_VolExit_validator_indices(ve[..|ve|-1]) ==> 0 <= i < |s.validators|; 
-
-            assert forall i :: i in get_VolExit_validator_indices(ve[..|ve|-1]) ==> !s.validators[i].slashed;
-            assert forall i :: i in get_VolExit_validator_indices(ve[..|ve|-1]) ==> s.validators[i].activation_epoch <= get_current_epoch(s) < s.validators[i].withdrawable_epoch;
-            assert forall i :: i in get_VolExit_validator_indices(ve[..|ve|-1]) ==> s.validators[i].exitEpoch == FAR_FUTURE_EPOCH;
-            assert forall i :: i in get_VolExit_validator_indices(ve[..|ve|-1]) ==> get_current_epoch(s) >= s.validators[i].activation_epoch + SHARD_COMMITTEE_PERIOD;
-            //assert forall i :: 0 <= i < |s.validators| && i !in get_VolExit_validator_indices(ve[..|ve|-1]) ==> 
-            //    updateVoluntaryExits(s,ve[..|ve|-1]).validators[i].exitEpoch == s.validators[i].exitEpoch;
-
-            // assert forall i :: 0 <= i < |s.validators| && i !in get_VolExit_validator_indices(ve[..|ve|-1]) ==> updateVoluntaryExits(s, ve[..|ve|-1]).validators[i].slashed == s.validators[i].slashed;
-            // assert ve[|ve|-1].validator_index as int !in get_VolExit_validator_indices(ve[..|ve|-1]) ==> 
-            //     updateVoluntaryExits(s, ve[..|ve|-1]).validators[ve[|ve|-1].validator_index].slashed  == s.validators[ve[|ve|-1].validator_index].slashed;
-            // assert !s.validators[ve[|ve|-1].validator_index].slashed;
-
-            // assert forall i :: 0 <= i < |s.validators| && i !in get_VolExit_validator_indices(ve[..|ve|-1]) ==> updateVoluntaryExits(s, ve[..|ve|-1]).validators[i].exitEpoch == s.validators[i].exitEpoch;
-            // assert ve[|ve|-1].validator_index as int !in get_VolExit_validator_indices(ve[..|ve|-1]) ==> 
-            //     updateVoluntaryExits(s, ve[..|ve|-1]).validators[ve[|ve|-1].validator_index].exitEpoch  == s.validators[ve[|ve|-1].validator_index].exitEpoch;
-            // assert ve[|ve|-1].validator_index as int in get_VolExit_validator_indices(ve) ==> s.validators[ve[|ve|-1].validator_index].exitEpoch == FAR_FUTURE_EPOCH;
-
-            assert |updateVoluntaryExits(s,ve[..|ve|-1]).validators| == |s.validators|;
-            mappingVolExitIndices(ve);
-            subsetMappingVolExitIndices(ve, |ve|-1);
-            //assume ve[|ve|-1].validator_index as int < |updateVoluntaryExits(s,ve[..|ve|-1]).validators|;
-            //assert forall i :: i in get_VolExit_validator_indices(ve) ==> i < |s.validators|;  // from requires
-            assert ve[|ve|-1].validator_index as int in get_VolExit_validator_indices(ve);
-
-            //assume get_current_epoch(updateVoluntaryExits(s,ve[..|ve|-1])) >= ve[|ve|-1].epoch;
-            assert get_current_epoch(updateVoluntaryExits(s,ve[..|ve|-1])) == get_current_epoch(s);
-            assert get_current_epoch(s) >= ve[|ve|-1].epoch; // from requires
-
-            //helperVoluntaryExitLemma(updateVoluntaryExits(s,ve[..|ve|-1]), ve[|ve|-1]);
-            updateVoluntaryExit(updateVoluntaryExits(s,ve[..|ve|-1]), ve[|ve|-1])
-    }
-
-    
-    // function updateProposerSlashing(s: BeaconState, ps : ProposerSlashing) : BeaconState 
-    //     requires ps.header_1.slot == ps.header_2.slot
-    //     requires ps.header_1.proposer_index == ps.header_2.proposer_index 
-    //     requires ps.header_1 == ps.header_2
-    //     requires ps.header_1.proposer_index as int < |s.validators| 
-    //     //requires is_slashable_validator(s.validators[ps.header_1.proposer_index], get_current_epoch(s));
-    //     requires !s.validators[ps.header_1.proposer_index].slashed
-    //     requires s.validators[ps.header_1.proposer_index].activation_epoch <= get_current_epoch(s) < s.validators[ps.header_1.proposer_index].withdrawable_epoch
-
-    //     requires |get_active_validator_indices(s.validators, get_current_epoch(s))| > 0
-    //     requires |s.validators| == |s.balances|
-
-    //     ensures |s.validators| == |updateProposerSlashing(s, ps).validators| 
-    //     ensures |s.balances| == |updateProposerSlashing(s, ps).balances| 
-        
-    //     ensures forall i :: 0 <= i < |s.validators| && i != ps.header_1.proposer_index as int ==> updateProposerSlashing(s, ps).validators[i] == s.validators[i]
-    //     // ensures forall i :: 0 <= i < |s.validators| && i != ps.header_1.proposer_index as int ==> updateProposerSlashing(s, ps).validators[i].exitEpoch == s.validators[i].exitEpoch
-    //     // ensures forall i :: 0 <= i < |s.validators| && i != ps.header_1.proposer_index as int ==> updateProposerSlashing(s, ps).validators[i].withdrawable_epoch == s.validators[i].withdrawable_epoch
-    //     // ensures forall i :: 0 <= i < |s.validators| && i != ps.header_1.proposer_index as int ==> updateProposerSlashing(s, ps).validators[i].slashed == s.validators[i].slashed
-
-
-    //     ensures updateProposerSlashing(s, ps) == slash_validator(s, ps.header_1.proposer_index, get_beacon_proposer_index(s))
-    //     ensures get_current_epoch(updateProposerSlashing(s, ps)) == get_current_epoch(s)
-    //     ensures forall i :: 0 <= i < |s.validators| ==> updateProposerSlashing(s, ps).validators[i].activation_epoch == s.validators[i].activation_epoch
-       
-    //     ensures updateProposerSlashing(s, ps).slot == s.slot
-    //     ensures updateProposerSlashing(s, ps).eth1_deposit_index == s.eth1_deposit_index
-    //     ensures updateProposerSlashing(s, ps).latest_block_header == s.latest_block_header
-        
-    //     //ensures get_current_epoch(s) >= updateVoluntaryExit(s, voluntary_exit).validators[voluntary_exit.validator_index].activation_epoch + SHARD_COMMITTEE_PERIOD 
-    // {
-    //     slash_validator(s, ps.header_1.proposer_index, get_beacon_proposer_index(s))
-    //     // maybe expand???
-    // }
-
-    
-
-    // function updateProposerSlashings(s: BeaconState, ps : seq<ProposerSlashing>) : BeaconState
-    //     requires minimumActiveValidators(s)
-    //     requires forall i,j :: 0 <= i < j < |ps| && i != j ==> ps[i].header_1.proposer_index!= ps[j].header_1.proposer_index // ve indices are unique
-        
-    //     requires forall i :: 0 <= i < |ps| ==> ps[i].header_1.slot == ps[i].header_2.slot
-    //     requires forall i :: 0 <= i < |ps| ==> ps[i].header_1.proposer_index == ps[i].header_2.proposer_index 
-    //     requires forall i :: 0 <= i < |ps| ==> ps[i].header_1 == ps[i].header_2
-    //     requires forall i :: 0 <= i < |ps| ==> ps[i].header_1.proposer_index as int < |s.validators| 
-    //     requires forall i :: 0 <= i < |ps| ==> !s.validators[ps[i].header_1.proposer_index].slashed 
-    //     requires forall i :: 0 <= i < |ps| ==> s.validators[ps[i].header_1.proposer_index].activation_epoch <= get_current_epoch(s) < s.validators[ps[i].header_1.proposer_index].withdrawable_epoch
-
-        
-    //     //requires forall i :: 0 <= i < |ps| ==> is_slashable_validator(s.validators[ps[i].header_1.proposer_index], get_current_epoch(s));
-    //     //requires forall i :: i in get_PS_validator_indices(ps) ==> 0 <= i < |s.validators| //this should be the same as the previous requires!
-    //     //requires forall i :: i in get_PS_validator_indices(ps) ==> !s.validators[i].slashed
-    //     //requires forall i :: i in get_PS_validator_indices(ps) ==> s.validators[i].activation_epoch <= get_current_epoch(s) < s.validators[i].withdrawable_epoch
-        
-        
-    //     //requires forall i :: 0 <= i < |ps| ==> !s.validators[ps[i].header_1.proposer_index].slashed
-    //     //requires forall i :: 0 <= i < |ps| ==> s.validators[ps[i].header_1.proposer_index].activation_epoch <= get_current_epoch(s) < s.validators[ps[i].header_1.proposer_index].withdrawable_epoch
-
-
-    //     //requires forall i :: 0 <= i < |ps| ==> s.validators[ps[i].header_1.proposer_index].exitEpoch == FAR_FUTURE_EPOCH
-    //     // not required for proposer slashings (but is for vol exits)
-    //     requires |get_active_validator_indices(s.validators, get_current_epoch(s))| > 0
-    //     requires |s.validators| == |s.balances|
-
-    //     ensures |updateProposerSlashings(s, ps).validators| == |s.validators|
-    //     ensures |updateProposerSlashings(s, ps).validators| == |updateProposerSlashings(s, ps).balances|
-
-    //     ensures get_current_epoch(updateProposerSlashings(s, ps)) == get_current_epoch(s)
-    //     ensures forall i :: 0 <= i < |s.validators| ==> updateProposerSlashings(s, ps).validators[i].activation_epoch == s.validators[i].activation_epoch
-    //     //ensures forall i :: 0 <= i < |s.validators| ==> forall j :: 0 <= j < |ps| && i != ps[j].header_1.proposer_index as int ==> updateProposerSlashings(s, ps).validators[i].exitEpoch == s.validators[i].exitEpoch
-    //     //ensures forall i :: 0 <= i < |s.validators| ==> forall j :: 0 <= j < |ps| && i != ps[j].header_1.proposer_index as int ==> updateProposerSlashings(s, ps).validators[i].withdrawable_epoch == s.validators[i].withdrawable_epoch
-    //     //ensures forall i :: 0 <= i < |s.validators| ==> forall j :: 0 <= j < |ps| && i != ps[j].header_1.proposer_index as int ==> updateProposerSlashings(s, ps).validators[i].slashed == s.validators[i].slashed
-
-    //     ensures |get_active_validator_indices(updateProposerSlashings(s, ps).validators, get_current_epoch(s))| > 0
-    //     ensures forall i :: 0 <= i < |s.validators| && i !in get_PS_validator_indices(ps) ==> updateProposerSlashings(s, ps).validators[i] == s.validators[i]
-        
-
-    //     ensures updateProposerSlashings(s, ps).slot == s.slot
-    //     ensures updateProposerSlashings(s, ps).eth1_deposit_index == s.eth1_deposit_index
-    //     ensures updateProposerSlashings(s, ps).latest_block_header == s.latest_block_header
-    //     ensures minimumActiveValidators(updateProposerSlashings(s, ps))
-
-    //     decreases |ps|
-
-    // {
-    //     if |ps| == 0 then s
-    //     else
-    //         helperPSLemma3(s, ps);
-    //         helperPSLemma2(s, ps);
-    //         assert forall i :: i in get_PS_validator_indices(ps[..|ps|-1]) ==> 0 <= i < |s.validators|; 
-    //         assert forall i :: i in get_PS_validator_indices(ps[..|ps|-1]) ==> !s.validators[i].slashed;
-    //         assert forall i :: i in get_PS_validator_indices(ps[..|ps|-1]) ==> s.validators[i].activation_epoch <= get_current_epoch(s) < s.validators[i].withdrawable_epoch;
-    //         //assert forall i :: i in get_PS_validator_indices(ps[..|ps|-1]) ==> get_current_epoch(s) >= s.validators[i].activation_epoch + SHARD_COMMITTEE_PERIOD;
-    //         assert |updateProposerSlashings(s,ps[..|ps|-1]).validators| == |s.validators|;
-    //         mappingPSIndices(ps);
-    //         subsetMappingPSIndices(ps, |ps|-1);
-    //         //assume ve[|ve|-1].validator_index as int < |updateVoluntaryExits(s,ve[..|ve|-1]).validators|;
-    //         //assert forall i :: i in get_VolExit_validator_indices(ve) ==> i < |s.validators|;  // from requires
-    //         assert ps[|ps|-1].header_1.proposer_index as int in get_PS_validator_indices(ps);
-
-    //         //assume get_current_epoch(updateVoluntaryExits(s,ve[..|ve|-1])) >= ve[|ve|-1].epoch;
-    //         assert get_current_epoch(updateProposerSlashings(s,ps[..|ps|-1])) == get_current_epoch(s);
-            
-    //         //assert get_current_epoch(s) >= ps[|ps|-1].epoch; // from requires
-
-    //         //helperPSLemma(updateProposerSlashings(s,ps[..|ps|-1]), ps[|ps|-1]);
-    //         // var s1 := updateProposerSlashings(s,ps[..|ps|-1]);
-    //         // var last_ps := ps[|ps|-1];
-    //         // assert forall i :: 0 <= i < |s1.validators| && i != last_ps.header_1.proposer_index as int ==> updateProposerSlashing(s1, last_ps).validators[i].exitEpoch == s1.validators[i].exitEpoch;
-    //         // assert forall i :: 0 <= i < |s1.validators| && i != last_ps.header_1.proposer_index as int ==> updateProposerSlashing(s1, last_ps).validators[i].slashed == s1.validators[i].slashed;
-    //         // assert forall i :: 0 <= i < |s1.validators| && i != last_ps.header_1.proposer_index as int ==> updateProposerSlashing(s1, last_ps).validators[i].withdrawable_epoch == s1.validators[i].withdrawable_epoch;
-    
-    //         //** try incorporating this next and whether helpePSLemma then follows */
-            
-    //         updateProposerSlashingLemma(updateProposerSlashings(s,ps[..|ps|-1]), ps[|ps|-1]);
-    //         //ensures |get_active_validator_indices(updateProposerSlashing(s, ps).validators, get_current_epoch(s))| > 0
-
-    //         updateProposerSlashing(updateProposerSlashings(s,ps[..|ps|-1]), ps[|ps|-1])
-
-    // }
-
-
-    
-
-
-
-    function updateProposerSlashing(s: BeaconState, ps : ProposerSlashing) : BeaconState 
+     function updateProposerSlashing(s: BeaconState, ps : ProposerSlashing) : BeaconState 
+        // |get_active_validator_indices(s.validators, get_current_epoch(s))| > 0
         requires minimumActiveValidators(s)
         requires ps.header_1.slot == ps.header_2.slot
         requires ps.header_1.proposer_index == ps.header_2.proposer_index 
@@ -803,135 +312,97 @@ module ProcessOperationsSpec {
         requires ps.header_1.proposer_index as int < |s.validators| 
         //requires is_slashable_validator(s.validators[ps.header_1.proposer_index], get_current_epoch(s));
         requires !s.validators[ps.header_1.proposer_index].slashed
-        requires s.validators[ps.header_1.proposer_index].activation_epoch <= get_current_epoch(s) < s.validators[ps.header_1.proposer_index].withdrawable_epoch
-
-        //requires |get_active_validator_indices(s.validators, get_current_epoch(s))| > 0
+        requires s.validators[ps.header_1.proposer_index].activation_epoch 
+                    <= get_current_epoch(s) 
+                    < s.validators[ps.header_1.proposer_index].withdrawable_epoch
         requires |s.validators| == |s.balances|
 
         ensures |s.validators| == |updateProposerSlashing(s, ps).validators| 
         ensures |s.balances| == |updateProposerSlashing(s, ps).balances| 
-        
-        ensures forall i :: 0 <= i < |s.validators| && i != ps.header_1.proposer_index as int ==> updateProposerSlashing(s, ps).validators[i] == s.validators[i]
-        // ensures forall i :: 0 <= i < |s.validators| && i != ps.header_1.proposer_index as int ==> updateProposerSlashing(s, ps).validators[i].exitEpoch == s.validators[i].exitEpoch
-        // ensures forall i :: 0 <= i < |s.validators| && i != ps.header_1.proposer_index as int ==> updateProposerSlashing(s, ps).validators[i].withdrawable_epoch == s.validators[i].withdrawable_epoch
-        // ensures forall i :: 0 <= i < |s.validators| && i != ps.header_1.proposer_index as int ==> updateProposerSlashing(s, ps).validators[i].slashed == s.validators[i].slashed
-
-
-        //ensures updateProposerSlashing(s, ps) == slash_validator(s, ps.header_1.proposer_index, get_beacon_proposer_index(s))
+        ensures forall i :: 0 <= i < |s.validators| && i != ps.header_1.proposer_index as int 
+                    ==> updateProposerSlashing(s, ps).validators[i] 
+                        == s.validators[i]
+        ensures updateProposerSlashing(s, ps) 
+                == slash_validator(s, ps.header_1.proposer_index, get_beacon_proposer_index(s))
         ensures get_current_epoch(updateProposerSlashing(s, ps)) == get_current_epoch(s)
-        ensures forall i :: 0 <= i < |s.validators| ==> updateProposerSlashing(s, ps).validators[i].activation_epoch == s.validators[i].activation_epoch
-       
+        ensures forall i :: 0 <= i < |s.validators| 
+                    ==> updateProposerSlashing(s, ps).validators[i].activation_epoch 
+                        == s.validators[i].activation_epoch
         ensures updateProposerSlashing(s, ps).slot == s.slot
         ensures updateProposerSlashing(s, ps).eth1_deposit_index == s.eth1_deposit_index
         ensures updateProposerSlashing(s, ps).latest_block_header == s.latest_block_header
-
         ensures minimumActiveValidators(updateProposerSlashing(s, ps))
-        
-        //ensures get_current_epoch(s) >= updateVoluntaryExit(s, voluntary_exit).validators[voluntary_exit.validator_index].activation_epoch + SHARD_COMMITTEE_PERIOD 
     {
         var s' := slash_validator(s, ps.header_1.proposer_index, get_beacon_proposer_index(s));
-        slashValidatorPreservesMinimumActiveValidators(s, ps.header_1.proposer_index, get_beacon_proposer_index(s));
+        // lemma to ensure minimumActiveValidators(updateProposerSlashing(s, ps))
+        slashValidatorPreservesMinimumActiveValidators(s, 
+                                                      ps.header_1.proposer_index, 
+                                                      get_beacon_proposer_index(s));
         s'
     }
 
-    
-
+    /**
+     *  The functional equivalent of processing a sequence of proposer slashings.
+     *  
+     *  @param  s       A beacon state.
+     *  @param  ps      A sequence of proposer slashings. 
+     *  @returns        A new state obtained from processing ps.        
+     */
     function updateProposerSlashings(s: BeaconState, ps : seq<ProposerSlashing>) : BeaconState
         requires minimumActiveValidators(s)
-        requires forall i,j :: 0 <= i < j < |ps| && i != j ==> ps[i].header_1.proposer_index!= ps[j].header_1.proposer_index // ve indices are unique
-        
+        requires forall i,j :: 0 <= i < j < |ps| && i != j // indices are unique
+            ==> ps[i].header_1.proposer_index != ps[j].header_1.proposer_index 
         requires forall i :: 0 <= i < |ps| ==> ps[i].header_1.slot == ps[i].header_2.slot
-        requires forall i :: 0 <= i < |ps| ==> ps[i].header_1.proposer_index == ps[i].header_2.proposer_index 
+        requires forall i :: 0 <= i < |ps| 
+                    ==> ps[i].header_1.proposer_index == ps[i].header_2.proposer_index 
         requires forall i :: 0 <= i < |ps| ==> ps[i].header_1 == ps[i].header_2
         requires forall i :: 0 <= i < |ps| ==> ps[i].header_1.proposer_index as int < |s.validators| 
         requires forall i :: 0 <= i < |ps| ==> !s.validators[ps[i].header_1.proposer_index].slashed 
-        requires forall i :: 0 <= i < |ps| ==> s.validators[ps[i].header_1.proposer_index].activation_epoch <= get_current_epoch(s) < s.validators[ps[i].header_1.proposer_index].withdrawable_epoch
-
-        //requires |get_active_validator_indices(s.validators, get_current_epoch(s))| > 0
+        requires forall i :: 0 <= i < |ps| 
+                    ==> s.validators[ps[i].header_1.proposer_index].activation_epoch 
+                        <= get_current_epoch(s) 
+                        < s.validators[ps[i].header_1.proposer_index].withdrawable_epoch
         requires |s.validators| == |s.balances|
-        //requires forall i :: 0 <= i < |ps| ==> is_slashable_validator(s.validators[ps[i].header_1.proposer_index], get_current_epoch(s));
-        //requires forall i :: i in get_PS_validator_indices(ps) ==> 0 <= i < |s.validators| //this should be the same as the previous requires!
-        //requires forall i :: i in get_PS_validator_indices(ps) ==> !s.validators[i].slashed
-        //requires forall i :: i in get_PS_validator_indices(ps) ==> s.validators[i].activation_epoch <= get_current_epoch(s) < s.validators[i].withdrawable_epoch
-        
-        
-        //requires forall i :: 0 <= i < |ps| ==> !s.validators[ps[i].header_1.proposer_index].slashed
-        //requires forall i :: 0 <= i < |ps| ==> s.validators[ps[i].header_1.proposer_index].activation_epoch <= get_current_epoch(s) < s.validators[ps[i].header_1.proposer_index].withdrawable_epoch
-
-
-        //requires forall i :: 0 <= i < |ps| ==> s.validators[ps[i].header_1.proposer_index].exitEpoch == FAR_FUTURE_EPOCH
-        // not required for proposer slashings (but is for vol exits)
         
         ensures updateProposerSlashings(s, ps).slot == s.slot
         //ensures get_current_epoch(updateProposerSlashings(s, ps)) == get_current_epoch(s)
-
         ensures updateProposerSlashings(s, ps).eth1_deposit_index == s.eth1_deposit_index
         ensures updateProposerSlashings(s, ps).latest_block_header == s.latest_block_header
-
-        ensures minimumActiveValidators(updateProposerSlashings(s, ps))
-        //ensures |get_active_validator_indices(updateProposerSlashings(s, ps).validators, get_current_epoch(s))| > 0
-        
         ensures |updateProposerSlashings(s, ps).validators| == |s.validators|
         ensures |updateProposerSlashings(s, ps).validators| == |updateProposerSlashings(s, ps).balances|
+        ensures forall i :: 0 <= i < |s.validators| 
+                    ==> updateProposerSlashings(s, ps).validators[i].activation_epoch 
+                        == s.validators[i].activation_epoch
+        ensures forall i :: 0 <= i < |s.validators| && i !in get_PS_validator_indices(ps) 
+                    ==> updateProposerSlashings(s, ps).validators[i] 
+                        == s.validators[i]
+        ensures minimumActiveValidators(updateProposerSlashings(s, ps))
 
-        ensures forall i :: 0 <= i < |s.validators| ==> updateProposerSlashings(s, ps).validators[i].activation_epoch == s.validators[i].activation_epoch
-        //ensures forall i :: 0 <= i < |s.validators| ==> forall j :: 0 <= j < |ps| && i != ps[j].header_1.proposer_index as int ==> updateProposerSlashings(s, ps).validators[i].exitEpoch == s.validators[i].exitEpoch
-        //ensures forall i :: 0 <= i < |s.validators| ==> forall j :: 0 <= j < |ps| && i != ps[j].header_1.proposer_index as int ==> updateProposerSlashings(s, ps).validators[i].withdrawable_epoch == s.validators[i].withdrawable_epoch
-        //ensures forall i :: 0 <= i < |s.validators| ==> forall j :: 0 <= j < |ps| && i != ps[j].header_1.proposer_index as int ==> updateProposerSlashings(s, ps).validators[i].slashed == s.validators[i].slashed
-
-        ensures forall i :: 0 <= i < |s.validators| && i !in get_PS_validator_indices(ps) ==> updateProposerSlashings(s, ps).validators[i] == s.validators[i]
-        
-
-        
         decreases |ps|
-
     {
         if |ps| == 0 then s
         else
-            // helperPSLemma3(s, ps);
-            // helperPSLemma2(s, ps);
-            // assert forall i :: i in get_PS_validator_indices(ps[..|ps|-1]) ==> 0 <= i < |s.validators|; 
-            // assert forall i :: i in get_PS_validator_indices(ps[..|ps|-1]) ==> !s.validators[i].slashed;
-            // assert forall i :: i in get_PS_validator_indices(ps[..|ps|-1]) ==> s.validators[i].activation_epoch <= get_current_epoch(s) < s.validators[i].withdrawable_epoch;
-            // //assert forall i :: i in get_PS_validator_indices(ps[..|ps|-1]) ==> get_current_epoch(s) >= s.validators[i].activation_epoch + SHARD_COMMITTEE_PERIOD;
-            // assert |updateProposerSlashings(s,ps[..|ps|-1]).validators| == |s.validators|;
-            // mappingPSIndices(ps);
-            // subsetMappingPSIndices(ps, |ps|-1);
-            // //assume ve[|ve|-1].validator_index as int < |updateVoluntaryExits(s,ve[..|ve|-1]).validators|;
-            // //assert forall i :: i in get_VolExit_validator_indices(ve) ==> i < |s.validators|;  // from requires
-            // assert ps[|ps|-1].header_1.proposer_index as int in get_PS_validator_indices(ps);
-
-            // //assume get_current_epoch(updateVoluntaryExits(s,ve[..|ve|-1])) >= ve[|ve|-1].epoch;
-            // assert get_current_epoch(updateProposerSlashings(s,ps[..|ps|-1])) == get_current_epoch(s);
-
-
-            
-            //assert get_current_epoch(s) >= ps[|ps|-1].epoch; // from requires
-
-            //helperPSLemma(updateProposerSlashings(s,ps[..|ps|-1]), ps[|ps|-1]);
-            // var s1 := updateProposerSlashings(s,ps[..|ps|-1]);
-            // var last_ps := ps[|ps|-1];
-            // assert forall i :: 0 <= i < |s1.validators| && i != last_ps.header_1.proposer_index as int ==> updateProposerSlashing(s1, last_ps).validators[i].exitEpoch == s1.validators[i].exitEpoch;
-            // assert forall i :: 0 <= i < |s1.validators| && i != last_ps.header_1.proposer_index as int ==> updateProposerSlashing(s1, last_ps).validators[i].slashed == s1.validators[i].slashed;
-            // assert forall i :: 0 <= i < |s1.validators| && i != last_ps.header_1.proposer_index as int ==> updateProposerSlashing(s1, last_ps).validators[i].withdrawable_epoch == s1.validators[i].withdrawable_epoch;
-    
-            //** try incorporating this next and whether helpePSLemma then follows */
-
-            //updateProposerSlashingLemma(updateProposerSlashings(s,ps[..|ps|-1]), ps[|ps|-1]);
-            //ensures |get_active_validator_indices(updateProposerSlashing(s, ps).validators, get_current_epoch(s))| > 0
-
             // preconditions for updateProposerSlashings
             assert minimumActiveValidators(s);
             var ps1 := ps[..|ps|-1];
             assert forall i :: 0 <= i < |ps1| ==> ps1[i] == ps[i];
-            assert forall i,j :: 0 <= i < j < |ps1| && i != j ==> ps1[i].header_1.proposer_index!= ps1[j].header_1.proposer_index; // ve indices are unique
+            assert forall i,j :: 0 <= i < j < |ps1| && i != j // ve indices are unique
+                        ==> ps1[i].header_1.proposer_index != ps1[j].header_1.proposer_index; 
             
-            assert forall i :: 0 <= i < |ps1| ==> ps1[i].header_1.slot == ps1[i].header_2.slot; //== ps[i].header_1.slot == ps[i].header_2.slot;
-            assert forall i :: 0 <= i < |ps1| ==> ps1[i].header_1.proposer_index == ps1[i].header_2.proposer_index ;
-            assert forall i :: 0 <= i < |ps1| ==> ps1[i].header_1 == ps1[i].header_2;
-            assert forall i :: 0 <= i < |ps1| ==> ps1[i].header_1.proposer_index as nat < |s.validators| ;
-            assert forall i :: 0 <= i < |ps1| ==> !s.validators[ps1[i].header_1.proposer_index].slashed ;
-            assert forall i :: 0 <= i < |ps1| ==> s.validators[ps1[i].header_1.proposer_index].activation_epoch <= get_current_epoch(s) < s.validators[ps1[i].header_1.proposer_index].withdrawable_epoch;
+            assert forall i :: 0 <= i < |ps1| 
+                        ==> ps1[i].header_1.slot == ps1[i].header_2.slot; 
+            assert forall i :: 0 <= i < |ps1| 
+                        ==> ps1[i].header_1.proposer_index == ps1[i].header_2.proposer_index ;
+            assert forall i :: 0 <= i < |ps1| 
+                        ==> ps1[i].header_1 == ps1[i].header_2;
+            assert forall i :: 0 <= i < |ps1| 
+                        ==> ps1[i].header_1.proposer_index as nat < |s.validators| ;
+            assert forall i :: 0 <= i < |ps1| 
+                        ==> !s.validators[ps1[i].header_1.proposer_index].slashed ;
+            assert forall i :: 0 <= i < |ps1| 
+                        ==> s.validators[ps1[i].header_1.proposer_index].activation_epoch 
+                            <= get_current_epoch(s) 
+                            < s.validators[ps1[i].header_1.proposer_index].withdrawable_epoch;
 
             //requires |get_active_validator_indices(s.validators, get_current_epoch(s))| > 0
             assert |s.validators| == |s.balances|;
@@ -950,8 +421,10 @@ module ProcessOperationsSpec {
             assert |s1.validators| == |s.validators|;
             assert |s1.validators| == |s1.balances|;
 
-            assert forall i :: 0 <= i < |s.validators| ==> s1.validators[i].activation_epoch == s.validators[i].activation_epoch;
-            assert forall i :: 0 <= i < |s.validators| && i !in get_PS_validator_indices(ps1) ==> s1.validators[i] == s.validators[i];
+            assert forall i :: 0 <= i < |s.validators| 
+                        ==> s1.validators[i].activation_epoch == s.validators[i].activation_epoch;
+            assert forall i :: 0 <= i < |s.validators| && i !in get_PS_validator_indices(ps1) 
+                        ==> s1.validators[i] == s.validators[i];
 
             var ps2 := ps[|ps|-1];
 
@@ -959,138 +432,71 @@ module ProcessOperationsSpec {
             assert ps2.header_1.slot == ps2.header_2.slot;
             assert ps2.header_1.proposer_index == ps2.header_2.proposer_index ;
             assert ps2.header_1 == ps2.header_2;
-            assert ps2.header_1.proposer_index as int < |s1.validators| == |s.validators| ;
+            assert ps2.header_1.proposer_index as int < |s1.validators| == |s.validators|;
             
             assert ps2 !in ps1;
-            // seqInitLast<ProposerSlashing>(ps, |ps|-1);
-            // assert ps[..|ps|-1] + [ps[|ps|-1]] == ps[..|ps|];
-            // assert ps[..|ps|] == ps;
-            // assert ps1 + [ps2] == ps;
-            
-            testLemma1(s, s1, ps1, ps2, ps);
-            assert s1.validators[ps2.header_1.proposer_index] == s.validators[ps2.header_1.proposer_index];
+            PSHelperLemma1(s, s1, ps1, ps2, ps);
+            assert s1.validators[ps2.header_1.proposer_index] 
+                    == s.validators[ps2.header_1.proposer_index];
             assert !s1.validators[ps2.header_1.proposer_index].slashed;
-            assert s1.validators[ps2.header_1.proposer_index].activation_epoch <= get_current_epoch(s1) == get_current_epoch(s) < s1.validators[ps2.header_1.proposer_index].withdrawable_epoch;
-
-            //requires |get_active_validator_indices(s.validators, get_current_epoch(s))| > 0
+            assert s1.validators[ps2.header_1.proposer_index].activation_epoch 
+                    <= get_current_epoch(s1) == get_current_epoch(s) 
+                    < s1.validators[ps2.header_1.proposer_index].withdrawable_epoch;
             assert |s1.validators| == |s1.balances|;
 
-            
-            
-            
             //updateProposerSlashing(updateProposerSlashings(s,ps[..|ps|-1]), ps[|ps|-1])
             var s2 := updateProposerSlashing(s1, ps2);
-            
+
+            // check resulting post conditions of s2
             assert |s.validators| == |s2.validators| ;
             assert |s.balances| == |s2.balances| ;
-
-            //mappingPSIndices(ps);
-            //subsetMappingPSIndices(ps, |ps|-1);
         
-            assert forall i :: 0 <= i < |s.validators| && i !in get_PS_validator_indices(ps1) ==> s1.validators[i] == s.validators[i];
-            assert forall i :: 0 <= i < |s.validators| && i != ps2.header_1.proposer_index as int ==> s2.validators[i] == s1.validators[i];
-            assert forall i :: 0 <= i < |s.validators| && i !in get_PS_validator_indices(ps1) && i != ps2.header_1.proposer_index as int 
-                ==> s2.validators[i] == s.validators[i];
+            assert forall i :: 0 <= i < |s.validators| && i !in get_PS_validator_indices(ps1) 
+                        ==> s1.validators[i] == s.validators[i];
+            assert forall i :: 0 <= i < |s.validators| && i != ps2.header_1.proposer_index as int 
+                        ==> s2.validators[i] == s1.validators[i];
+            assert forall i :: 0 <= i < |s.validators| 
+                        && i !in get_PS_validator_indices(ps1) 
+                        && i != ps2.header_1.proposer_index as int 
+                        ==> s2.validators[i] == s.validators[i];
+            assert forall i :: 0 <= i < |s.validators| 
+                        && i !in (get_PS_validator_indices(ps1) + [ps2.header_1.proposer_index as int]) 
+                        ==> s2.validators[i] == s.validators[i];
 
-            assert forall i :: 0 <= i < |s.validators| && i !in (get_PS_validator_indices(ps1) + [ps2.header_1.proposer_index as int]) 
-                ==> s2.validators[i] == s.validators[i];
-
-            //assume get_PS_validator_indices(ps1) + [ps2.header_1.proposer_index as int] == get_PS_validator_indices(ps);
-            testLemma3(s, s2, ps1, ps2, ps);
-        
-            //testLemma2(s, ps1, ps2, ps);
-
-
-            //assume forall i :: i !in get_PS_validator_indices(ps1) && i != ps2.header_1.proposer_index as int 
-            //    ==>  i !in get_PS_validator_indices(ps);// ==> s2.validators[i] == s.validators[i];
-            
-            assert forall i :: 0 <= i < |s.validators| && i !in get_PS_validator_indices(ps) ==> s2.validators[i] == s.validators[i];
-        
-
-            //assert s2 == slash_validator(s, ps.header_1.proposer_index, get_beacon_proposer_index(s));
-            assert forall i :: 0 <= i < |s.validators| ==> s2.validators[i].activation_epoch == s.validators[i].activation_epoch;
+            PSHelperLemma2(s, s2, ps1, ps2, ps);
+            assert forall i :: 0 <= i < |s.validators| && i !in get_PS_validator_indices(ps) 
+                        ==> s2.validators[i] == s.validators[i];
+            assert forall i :: 0 <= i < |s.validators| 
+                        ==> s2.validators[i].activation_epoch == s.validators[i].activation_epoch;
        
             assert s2.slot == s.slot;
             assert s2.eth1_deposit_index == s.eth1_deposit_index;
             assert s2.latest_block_header == s.latest_block_header;
-
             assert minimumActiveValidators(s2);
-        
 
             s2
     }
 
-    
-
-    
-    /////////////////////////////////////////////////////////////////////////////////////
-
-    function updateAttesterSlashings(s: BeaconState, a: seq<AttesterSlashing>) : BeaconState 
-        requires forall i :: 0 <= i < |a| ==> is_valid_indexed_attestation(s, a[i].attestation_1)
-        requires forall i :: 0 <= i < |a| ==> is_valid_indexed_attestation(s, a[i].attestation_2)
-        requires forall i :: 0 <= i < |a| ==> forall j :: 0 <= j < |a[i].attestation_1.attesting_indices| ==> a[i].attestation_1.attesting_indices[j] as int < |s.validators|
-        requires forall i :: 0 <= i < |a| ==> forall j :: 0 <= j < |a[i].attestation_2.attesting_indices| ==> a[i].attestation_2.attesting_indices[j] as int < |s.validators|
-        //requires |get_active_validator_indices(s.validators, get_current_epoch(s))| > 0
-        requires minimumActiveValidators(s)
-        requires |s.validators| == |s.balances|
-
-        // explicitly show we only slash those n the intersection
-
-        ensures |s.validators| == |updateAttesterSlashings(s, a).validators| 
-        ensures |updateAttesterSlashings(s, a).validators| == |updateAttesterSlashings(s, a).balances| 
-        ensures updateAttesterSlashings(s, a).slot == s.slot
-        ensures updateAttesterSlashings(s, a).eth1_deposit_index == s.eth1_deposit_index
-        ensures updateAttesterSlashings(s, a).latest_block_header == s.latest_block_header
-       
-        //ensures |get_active_validator_indices(updateAttesterSlashings(s, a).validators, get_current_epoch(updateAttesterSlashings(s, a)))| > 0
-        ensures minimumActiveValidators(updateAttesterSlashings(s, a))
-        //decreases indices
-    {
-        if |a| == 0 then 
-            s
-        else  
-            updateAttesterSlashing(updateAttesterSlashings(s, a[..|a|-1]), sorted_intersection(a[|a|-1].attestation_1.attesting_indices, a[|a|-1].attestation_2.attesting_indices))
-
-    }
-
-    
-    
-    function updateAttesterSlashing(s: BeaconState, indices: seq<uint64>) : BeaconState 
-        
-        requires |get_active_validator_indices(s.validators, get_current_epoch(s))| > 0
-        requires |s.validators| == |s.balances|
-        requires valid_state_indices(s,indices)
-        //requires forall i :: 0 <= i < |indices| ==> indices[i] as int < |s.validators| 
-
-        ensures |s.validators| == |updateAttesterSlashing(s, indices).validators| 
-        ensures |updateAttesterSlashing(s, indices).validators| == |updateAttesterSlashing(s, indices).balances| 
-
-        
-        ensures updateAttesterSlashing(s, indices).slot == s.slot
-        ensures updateAttesterSlashing(s, indices).eth1_deposit_index == s.eth1_deposit_index
-        ensures updateAttesterSlashing(s, indices).latest_block_header == s.latest_block_header
-        
-        ensures |get_active_validator_indices(updateAttesterSlashing(s, indices).validators, get_current_epoch(updateAttesterSlashing(s, indices)))| > 0
-        decreases indices
-    {
-        if |indices| == 0 then 
-            s
-        else 
-            //slashValidatorPreservesActivateValidators(s, indices[|indices|-1], get_beacon_proposer_index(s));
-            updateAttesterSlashingComp(updateAttesterSlashing(s, indices[..|indices|-1]), indices[|indices|-1] as ValidatorIndex)
-            
-    }
-
+    /**
+     *  The functional equivalent of slashing validator[slash_index].
+     *  
+     *  @param  s               A beacon state.
+     *  @param  slash_index     A validator index. 
+     *  @returns                A new state obtained from slashing validator[slash_index].        
+     */
     function updateAttesterSlashingComp(s: BeaconState, slash_index: ValidatorIndex) : BeaconState 
         requires slash_index as int < |s.validators| 
         requires |get_active_validator_indices(s.validators, get_current_epoch(s))| > 0
         requires |s.validators| == |s.balances|
+
         ensures |updateAttesterSlashingComp(s, slash_index).validators| == |s.validators| 
-        ensures |updateAttesterSlashingComp(s, slash_index).validators| == |updateAttesterSlashingComp(s, slash_index).balances| 
+        ensures |updateAttesterSlashingComp(s, slash_index).validators| 
+                == |updateAttesterSlashingComp(s, slash_index).balances| 
         ensures updateAttesterSlashingComp(s, slash_index).slot == s.slot
         ensures updateAttesterSlashingComp(s, slash_index).eth1_deposit_index == s.eth1_deposit_index
-        
-        ensures |get_active_validator_indices(updateAttesterSlashingComp(s, slash_index).validators, get_current_epoch(updateAttesterSlashingComp(s, slash_index)))| > 0
+        ensures 
+            var s1 := updateAttesterSlashingComp(s, slash_index);
+            |get_active_validator_indices(s1.validators, get_current_epoch(s1))| > 0
     {
         if is_slashable_validator(s.validators[slash_index], get_current_epoch(s)) then
             slashValidatorPreservesActivateValidators(s, slash_index, get_beacon_proposer_index(s));
@@ -1098,390 +504,403 @@ module ProcessOperationsSpec {
         else
             s
     }
-
     
+    /**
+     *  The functional equivalent of processing a sequence of slashings.
+     *  
+     *  @param  s       A beacon state.
+     *  @param  indices A sequence of validator indices (as uint64) to be slashed. 
+     *  @returns        A new state obtained from slashing validator[indices[i]]
+     *                  for all 0 <= i < |indices|.        
+     */
+    function updateAttesterSlashing(s: BeaconState, indices: seq<uint64>) : BeaconState 
+        requires |get_active_validator_indices(s.validators, get_current_epoch(s))| > 0
+        requires |s.validators| == |s.balances|
+        requires valid_state_indices(s,indices)
+        //requires forall i :: 0 <= i < |indices| ==> indices[i] as int < |s.validators| 
 
-    
-//  //////////////////////////
-//  // Helper lemmas
+        ensures |s.validators| == |updateAttesterSlashing(s, indices).validators| 
+        ensures |updateAttesterSlashing(s, indices).validators| 
+                == |updateAttesterSlashing(s, indices).balances| 
+        ensures updateAttesterSlashing(s, indices).slot == s.slot
+        ensures updateAttesterSlashing(s, indices).eth1_deposit_index == s.eth1_deposit_index
+        ensures updateAttesterSlashing(s, indices).latest_block_header == s.latest_block_header
+        ensures 
+            var s1 := updateAttesterSlashing(s, indices);
+            |get_active_validator_indices(s1.validators, get_current_epoch(s1))| > 0
+        decreases indices
+    {
+        if |indices| == 0 then 
+            s
+        else 
+            updateAttesterSlashingComp(
+                updateAttesterSlashing(s, indices[..|indices|-1]), 
+                indices[|indices|-1] as ValidatorIndex
+            )
+    }
 
-//     lemma helperIndicesLemma(indices: seq<ValidatorIndex>)
-//         requires |indices| > 0
-//         ensures forall i :: 0 < i < |indices| ==> indices[..i+1] == indices[..i] + [indices[i]]
-//     {
-//         // Thanks Dafny
-//     }
+    /**
+     *  The functional equivalent of processing a sequence of attester slashings.
+     *  
+     *  @param  s       A beacon state.
+     *  @param  a       A sequence of attester slashings. 
+     *  @returns        A new state obtained from processing a.
+     *                  
+     *  @note           Three levels of functions are used instead of just two because the indices
+     *                  for slashing need to be extracted from a before recursion can be used.
+     *                  i.e. in  updateAttesterSlashings the indices are extracted, in 
+     *                  updateAttesterSlashing a sequence of indices are processed, and then in 
+     *                  updateAttesterSlashingComp an individual validator is slashed.
+     *  @note           For consistency the top two level functions have the naming conventions 
+     *                  used throughout.
+     *  @note           This function does not currently show that only those validators in
+     *                  the sorted intersection are slashed.
+     */
+    function updateAttesterSlashings(s: BeaconState, a: seq<AttesterSlashing>) : BeaconState 
+        requires forall i :: 0 <= i < |a| ==> is_valid_indexed_attestation(s, a[i].attestation_1)
+        requires forall i :: 0 <= i < |a| ==> is_valid_indexed_attestation(s, a[i].attestation_2)
+        requires forall i :: 0 <= i < |a| 
+                    ==> forall j :: 0 <= j < |a[i].attestation_1.attesting_indices|
+                    ==> a[i].attestation_1.attesting_indices[j] as int < |s.validators|
+        requires forall i :: 0 <= i < |a| 
+                    ==> forall j :: 0 <= j < |a[i].attestation_2.attesting_indices| 
+                    ==> a[i].attestation_2.attesting_indices[j] as int < |s.validators|
+        //requires |get_active_validator_indices(s.validators, get_current_epoch(s))| > 0
+        requires minimumActiveValidators(s)
+        requires |s.validators| == |s.balances|
 
-//     lemma helperIndicesLemma2(indices: seq<ValidatorIndex>)
-//         requires |indices| > 0
-//         ensures indices == indices[..|indices|-1] + [indices[|indices|-1]]
-//     {
-//         // Thanks Dafny
-//     }
+        ensures |s.validators| == |updateAttesterSlashings(s, a).validators| 
+        ensures |updateAttesterSlashings(s, a).validators| == |updateAttesterSlashings(s, a).balances| 
+        ensures updateAttesterSlashings(s, a).slot == s.slot
+        ensures updateAttesterSlashings(s, a).eth1_deposit_index == s.eth1_deposit_index
+        ensures updateAttesterSlashings(s, a).latest_block_header == s.latest_block_header
+        ensures minimumActiveValidators(updateAttesterSlashings(s, a))
+    {
+        if |a| == 0 then 
+            s
+        else  
+            updateAttesterSlashing(updateAttesterSlashings(s, a[..|a|-1]), 
+                                   sorted_intersection(a[|a|-1].attestation_1.attesting_indices, 
+                                   a[|a|-1].attestation_2.attesting_indices)
+                                  )
+    }
 
-//     lemma helperIndicesLemma3(indices: seq<uint64>, i: nat)
-//         requires 0 <= i < |indices|
-//         ensures indices[..i+1] == indices[..i] + [indices[i]]
-//     {
-//         // Thanks Dafny
-//     }
+    /**
+     *  The functional equivalent of process_attestation.
+     *  
+     *  @param  s       A beacon state.
+     *  @param  a       An pattestation. 
+     *  @returns        A new state obtained from processing an attestation.        
+     */
+    function updateAttestation(s: BeaconState, a: Attestation) : BeaconState
+        requires attestationIsWellFormed(s, a)
+        requires |s.current_epoch_attestations| < MAX_ATTESTATIONS as nat * SLOTS_PER_EPOCH as nat 
+        requires |s.previous_epoch_attestations| < MAX_ATTESTATIONS as nat * SLOTS_PER_EPOCH as nat 
+        requires minimumActiveValidators(s)
+        ensures minimumActiveValidators(updateAttestation(s, a))
+        ensures 
+            var s1 := updateAttestation(s, a);
+            |s1.current_epoch_attestations| + |s1.previous_epoch_attestations| 
+                == |s.current_epoch_attestations| + |s.previous_epoch_attestations| + 1
+        ensures |s.current_epoch_attestations| 
+                    <= |updateAttestation(s, a).current_epoch_attestations| 
+                    <= |s.current_epoch_attestations| + 1
+        ensures |s.previous_epoch_attestations| 
+                    <=|updateAttestation(s, a).previous_epoch_attestations| 
+                    <= |s.previous_epoch_attestations| + 1
+        ensures 
+            var s1 := updateAttestation(s, a);
+            s1 == s.(current_epoch_attestations := s1.current_epoch_attestations) 
+            || s1 == s.(previous_epoch_attestations := s1.previous_epoch_attestations)
+        ensures updateAttestation(s, a).validators == s.validators
+        ensures updateAttestation(s, a).balances == s.balances
+        ensures updateAttestation(s, a).slot == s.slot
+        ensures updateAttestation(s, a).current_justified_checkpoint 
+                == s.current_justified_checkpoint
+        ensures updateAttestation(s, a).previous_justified_checkpoint 
+                == s.previous_justified_checkpoint
+        ensures updateAttestation(s, a).eth1_deposit_index == s.eth1_deposit_index
+    {
+        // data = attestation.data
+        assert get_previous_epoch(s) <= a.data.target.epoch <=  get_current_epoch(s);
+        assert a.data.target.epoch == compute_epoch_at_slot(a.data.slot);
+        assert a.data.slot as nat + MIN_ATTESTATION_INCLUSION_DELAY as nat 
+                <= s.slot as nat 
+                <= a.data.slot as nat + SLOTS_PER_EPOCH as nat;
+        assert a.data.index < get_committee_count_per_slot(s, a.data.target.epoch);
 
-//     lemma helperIndicesLemma4(s: BeaconState, indices: seq<uint64>, i: nat)
-//         requires 0 <= i <= |indices|
-//         requires valid_state_indices(s, indices)
-//         ensures valid_state_indices(s, indices[..i])
-//     {
-//         // Thanks Dafny
-//     }
+        var committee := get_beacon_committee(s, a.data.slot, a.data.index);
+        assert |a.aggregation_bits| == |committee|;
 
-//     lemma helperIndicesLemma5(indices: seq<uint64>, i: nat)
-//         requires i <= |indices|
-//         ensures |indices[..i]| == i;
-//     {
-//         // Thanks Dafny
-//     }
+        var pending := PendingAttestation(
+            a.aggregation_bits, 
+            a.data, 
+            (s.slot - a.data.slot), 
+            get_beacon_proposer_index(s) 
+        );
 
-//     lemma helperIndicesLemma6(indices: seq<uint64>, i: nat)
-//         requires i == |indices|
-//         ensures indices[..i] == indices
-//     {
-//         // Thanks Dafny
-//     }
-
-//     lemma helperIndicesLemma7(indices: seq<uint64>, i: nat)
-//         requires i < |indices|
-//         ensures indices[..i+1] == indices[..i] + [indices[i]];
-//     {
-//         // Thanks Dafny
-//     }
-
-
-
-// // lemma updateBalTotalBySingleDeposit(s: BeaconState, d: Deposit)
-// //         requires s.eth1_deposit_index as int +  1 < 0x10000000000000000 
-// //         requires |s.validators| == |s.balances|
-// //         requires |s.validators| + 1 <= VALIDATOR_REGISTRY_LIMIT as int
-// //         requires total_balances(s.balances) + d.data.amount as int < 0x10000000000000000
+        if a.data.target.epoch == get_current_epoch(s) then
+            //  Add a to current attestations
+            assert a.data.source == s.current_justified_checkpoint;
+            s.(
+                current_epoch_attestations := s.current_epoch_attestations + [pending]
+            )
+            // s.current_epoch_attestations.append(pending_attestation)
         
-// //         ensures total_balances(updateDeposit(s,d).balances) == total_balances(s.balances) + d.data.amount as int < 0x10000000000000000
-// //         //ensures total_balances(updateDeposit(s,d).balances) == total_balances(s.balances) + total_deposits([d]) 
-// //     {
-// //         var pk := seqKeysInValidators(s.validators); 
-// //         if |s.balances| == 0 {
-// //             // Thanks Dafny
-// //         }
-// //         else {
-// //             if d.data.pubkey in pk {
-// //                 var index := get_validator_index(pk, d.data.pubkey);
-// //                 individualBalanceBoundMaintained(s.balances,d);
-// //                 //assert updateDeposit(s,d).balances ==  increase_balance(s,index,d.data.amount).balances;
-// //                 //assert increase_balance(s,index,d.data.amount).balances[index] == s.balances[index] + d.data.amount;
-// //                 //assert forall i :: 0 <= i < |s.balances| && i != index as int ==> increase_balance(s,index,d.data.amount).balances[i] == s.balances[i];
-// //                 //assert total_balances(updateDeposit(s,d).balances) == total_balances(increase_balance(s,index,d.data.amount).balances) ;
-// //                 updateExistingBalance(s, index, d.data.amount);
-// //                 //assert total_balances(updateDeposit(s,d).balances) == total_balances(s.balances) + d.data.amount as int ;
-// //             }
-// //             else {
-// //                 //assert updateDeposit(s,d).balances == s.balances + [d.data.amount];
-// //                 distBalancesProp(s.balances,[d.data.amount]);
-// //                 //assert total_balances(s.balances + [d.data.amount]) == total_balances(s.balances) + total_balances([d.data.amount]);
-// //             }
-// //         }
-// //     }
-
-
-// ///////////////////////////
-//     lemma mappingPSIndices(ps: seq<ProposerSlashing>)
-//         ensures forall i :: 0 <= i < |ps| ==> get_PS_validator_indices(ps)[i] == ps[i].header_1.proposer_index as int
-//     {
-//         //Thanks Dafny
-//     }
-
-//     lemma subsetMappingPSIndices(ps: seq<ProposerSlashing>, i : nat)
-//         requires 0 <= i < |ps|
-//         ensures get_PS_validator_indices(ps[..i]) == get_PS_validator_indices(ps)[..i]
-//     {
-//         if |ps| == 0 {}
-//         else {
-//             assert ps == ps[..i] + ps[i..];
+        else 
+            assert a.data.source == s.previous_justified_checkpoint;
+            s.(
+                previous_epoch_attestations := s.previous_epoch_attestations + [pending]
+            )
+            // s.previous_epoch_attestations.append(pending_attestation)
             
-//             mappingPSIndices(ps[..i]);
-//             assert forall j :: 0 <= j < |ps[..i]| ==> get_PS_validator_indices(ps[..i])[j] == ps[j].header_1.proposer_index as int;
+        // # Verify signature
+        // Not implemented as part of the simplificiation
+        //assert is_valid_indexed_attestation(s', get_indexed_attestation(s', a));
+    }
 
-//             mappingPSIndices(ps);
-//             assert forall j :: 0 <= j < |ps| ==> get_PS_validator_indices(ps)[j] == ps[j].header_1.proposer_index as int;
-//         }
-//     }
-
-//     lemma helperPSLemma(s: BeaconState, ps: ProposerSlashing)
-//         requires ps.header_1.slot == ps.header_2.slot
-//         requires ps.header_1.proposer_index == ps.header_2.proposer_index 
-//         requires ps.header_1 == ps.header_2
-//         requires ps.header_1.proposer_index as int < |s.validators| 
-
-//         // requires is_active_validator: (!v.slashed) && (v.activation_epoch <= epoch < v.withdrawable_epoch)
-//         requires !s.validators[ps.header_1.proposer_index].slashed
-//         requires s.validators[ps.header_1.proposer_index].activation_epoch <= get_current_epoch(s) < s.validators[ps.header_1.proposer_index].withdrawable_epoch
- 
-//         requires |get_active_validator_indices(s.validators, get_current_epoch(s))| > 0
-//         requires |s.validators| == |s.balances|
+    /**
+     *  The functional equivalent of processing a sequence of attestations.
+     *  
+     *  @param  s       A beacon state.
+     *  @param  a       A sequence of attestations. 
+     *  @returns        A new state obtained from processing a.        
+     */
+    function updateAttestations(s: BeaconState, a: seq<Attestation>) : BeaconState
+        requires |s.validators| == |s.balances|
+        requires |a| as nat <= MAX_ATTESTATIONS as nat
+        requires forall i:: 0 <= i < |a| ==> attestationIsWellFormed(s, a[i])
+        requires |s.current_epoch_attestations| as nat + |a| as nat 
+                    <= MAX_ATTESTATIONS as nat * SLOTS_PER_EPOCH as nat 
+        requires |s.previous_epoch_attestations| as nat + |a| as nat 
+                    <= MAX_ATTESTATIONS as nat * SLOTS_PER_EPOCH as nat 
+        requires minimumActiveValidators(s)
         
-//         ensures forall i :: 0 <= i < |s.validators| && i != ps.header_1.proposer_index as int ==> updateProposerSlashing(s, ps).validators[i].exitEpoch == s.validators[i].exitEpoch
-//         ensures forall i :: 0 <= i < |s.validators| && i != ps.header_1.proposer_index as int ==> updateProposerSlashing(s, ps).validators[i].slashed == s.validators[i].slashed
-//         ensures forall i :: 0 <= i < |s.validators| && i != ps.header_1.proposer_index as int ==> updateProposerSlashing(s, ps).validators[i].withdrawable_epoch == s.validators[i].withdrawable_epoch
-//     {
-//         // Thanks Dafny
-//     }
+        ensures |updateAttestations(s,a).validators| == |updateAttestations(s,a).balances|
+        ensures 
+                var s1 := updateAttestations(s,a);
+                |s1.current_epoch_attestations| + |s1.previous_epoch_attestations| 
+                == |s.current_epoch_attestations| + |s.previous_epoch_attestations| + |a|
+        ensures |updateAttestations(s,a).current_epoch_attestations| 
+                    <= |s.current_epoch_attestations| + |a|;
+        ensures |updateAttestations(s,a).previous_epoch_attestations| 
+                    <= |s.previous_epoch_attestations| + |a|;
+        ensures minimumActiveValidators(updateAttestations(s, a))
+        ensures updateAttestations(s, a).validators == s.validators
+        ensures updateAttestations(s, a).slot == s.slot
+        ensures updateAttestations(s, a).current_justified_checkpoint == s.current_justified_checkpoint
+        ensures updateAttestations(s, a).previous_justified_checkpoint == s.previous_justified_checkpoint
+        ensures updateAttestations(s, a).eth1_deposit_index == s.eth1_deposit_index
+    {
+        if |a| == 0 then s
+        else
+            var index := |a| - 1;
+            var s1 := updateAttestations(s,a[..index]);
 
-//     lemma helperPSLemma2(s: BeaconState, ps: seq<ProposerSlashing>)
-//         requires  |get_PS_validator_indices(ps)| > 0
-//         requires forall i :: i in get_PS_validator_indices(ps) ==> 0 <= i < |s.validators| 
-//         requires forall i :: i in get_PS_validator_indices(ps) ==> !s.validators[i].slashed
-//         requires forall i :: i in get_PS_validator_indices(ps) ==> s.validators[i].activation_epoch <= get_current_epoch(s) < s.validators[i].withdrawable_epoch
+            //assert attestationIsWellFormed(s1, a[index]);
+            AttestationHelperLemma(s, s1, a[index]);
+
+            updateAttestation(s1, a[index])
+    }
+
+    /**
+     *  Take into account a single deposit from a block.
+     *
+     *  @param  s       A beacon state.
+     *  @param  d       A single deposit.
+     *  @returns        The state obtained after taking account the deposit `d` from state `s` 
+     */
+    function updateDeposit(s: BeaconState, d: Deposit) : BeaconState 
+        requires s.eth1_deposit_index as int +  1 < 0x10000000000000000 
+        requires |s.validators| == |s.balances|
+        requires |s.validators| + 1 <= VALIDATOR_REGISTRY_LIMIT as int
+        requires total_balances(s.balances) + d.data.amount as int < 0x10000000000000000
         
-
-//         ensures forall i :: i in get_PS_validator_indices(ps[..|ps|-1]) ==> 0 <= i < |s.validators|
-//         ensures forall i :: i in get_PS_validator_indices(ps[..|ps|-1]) ==> !s.validators[i].slashed
-//         ensures forall i :: i in get_PS_validator_indices(ps[..|ps|-1]) ==> s.validators[i].activation_epoch <= get_current_epoch(s) < s.validators[i].withdrawable_epoch
-//     {
-//         mappingPSIndices(ps);
-//         assert forall i :: 0 <= i < |ps| ==> get_PS_validator_indices(ps)[i] == ps[i].header_1.proposer_index as int;
-
-//         subsetMappingPSIndices(ps, |ps|-1);
-//         assert get_PS_validator_indices(ps[..|ps|-1]) == get_PS_validator_indices(ps)[..|ps|-1];
+        ensures d.data.pubkey !in seqKeysInValidators(s.validators) 
+                ==> updateDeposit(s,d).validators == s.validators + [get_validator_from_deposit(d)]
+        ensures d.data.pubkey in seqKeysInValidators(s.validators)  
+                ==> updateDeposit(s,d).validators == s.validators 
+        ensures updateDeposit(s,d).eth1_deposit_index == s.eth1_deposit_index + 1
+        ensures |updateDeposit(s,d).validators| == |updateDeposit(s,d).balances|        
+        ensures |s.validators| <= |updateDeposit(s,d).validators| <= |s.validators| + 1 
+        ensures |s.balances| <= |updateDeposit(s,d).balances| <= |s.balances| + 1 
+        ensures forall i :: 0 <= i < |s.balances| 
+                ==> s.balances[i] <= updateDeposit(s,d).balances[i]
+        ensures total_balances(updateDeposit(s,d).balances) 
+                == total_balances(s.balances) + d.data.amount as int 
+                < 0x10000000000000000
+    {
+        var pk := seqKeysInValidators(s.validators); 
+        var k := d.data.pubkey;
         
-//         assert forall i :: i in get_PS_validator_indices(ps) ==> 0 <= i < |s.validators|; // from requires
-//         assert forall i :: 0 <= i < |ps| ==> get_PS_validator_indices(ps)[i] == ps[i].header_1.proposer_index as int;
-//         assert forall i :: 0 <= i < |ps| ==> ps[i].header_1.proposer_index as int in get_PS_validator_indices(ps) ;
-        
-//     }
-
-
-//     lemma updateProposerSlashingLemma(s: BeaconState, ps : ProposerSlashing)
-//         requires ps.header_1.slot == ps.header_2.slot
-//         requires ps.header_1.proposer_index == ps.header_2.proposer_index 
-//         requires ps.header_1 == ps.header_2
-//         requires ps.header_1.proposer_index as int < |s.validators| 
-//         //requires is_slashable_validator(s.validators[ps.header_1.proposer_index], get_current_epoch(s));
-//         //(!v.slashed) && (v.activation_epoch <= epoch < v.withdrawable_epoch)
-//         requires !s.validators[ps.header_1.proposer_index].slashed
-//         requires s.validators[ps.header_1.proposer_index].activation_epoch <= get_current_epoch(s) < s.validators[ps.header_1.proposer_index].withdrawable_epoch
-        
-//         requires |get_active_validator_indices(s.validators, get_current_epoch(s))| > 0
-//         requires |s.validators| == |s.balances|
-        
-//         ensures |get_active_validator_indices(updateProposerSlashing(s, ps).validators, get_current_epoch(s))| > 0
-//     {
-//         var index := ps.header_1.proposer_index; // validator to be slashed
-//         var slashable_validator := s.validators[index];
-//         var epoch : Epoch := get_current_epoch(s);
-
-//         assert updateProposerSlashing(s, ps) == slash_validator(s, ps.header_1.proposer_index, get_beacon_proposer_index(s));
-//         slashValidatorPreservesActivateValidators(s, ps.header_1.proposer_index, get_beacon_proposer_index(s));
-//         assert |get_active_validator_indices(updateProposerSlashing(s, ps).validators, get_current_epoch(s))| > 0;
-
-//     }
-
-//     lemma helperPSLemma3(s: BeaconState, ps : seq<ProposerSlashing>)
-//         requires forall i :: 0 <= i < |ps| ==> ps[i].header_1.proposer_index as int < |s.validators| 
-//         requires forall i :: 0 <= i < |ps| ==> !s.validators[ps[i].header_1.proposer_index].slashed 
-//         requires forall i :: 0 <= i < |ps| ==> s.validators[ps[i].header_1.proposer_index].activation_epoch <= get_current_epoch(s) < s.validators[ps[i].header_1.proposer_index].withdrawable_epoch
-
-//         ensures forall i :: i in get_PS_validator_indices(ps) ==> 0 <= i < |s.validators|
-//         ensures forall i :: i in get_PS_validator_indices(ps) ==> !s.validators[i].slashed
-//         ensures forall i :: i in get_PS_validator_indices(ps) ==> s.validators[i].activation_epoch <= get_current_epoch(s) < s.validators[i].withdrawable_epoch
-//     {
-//         // Thanks Dafny
-//     }
-
-//     lemma helperPSLemma4(ps : seq<ProposerSlashing>)
-//         requires |ps| > 0
-//         requires forall i,j :: 0 <= i < j < |ps| && i != j ==> ps[i].header_1.proposer_index!= ps[j].header_1.proposer_index // ve indices are unique
-//         ensures ps[|ps|-1].header_1.proposer_index as int !in get_PS_validator_indices(ps[..|ps|-1])
-//     {
-//         mappingPSIndices(ps[..|ps|-1]);
-//         assert forall i :: 0 <= i < |ps[..|ps|-1]| ==> get_PS_validator_indices(ps[..|ps|-1])[i] == ps[i].header_1.proposer_index as int;
-//     }
-
-//     lemma helperPSLemma5(s: BeaconState, ps : seq<ProposerSlashing>)
-//         requires |ps| > 0
-//         requires forall i,j :: 0 <= i < j < |ps| && i != j ==> ps[i].header_1.proposer_index!= ps[j].header_1.proposer_index // ve indices are unique
-//         requires forall i :: 0 <= i < |ps| ==> ps[i].header_1.slot == ps[i].header_2.slot
-//         requires forall i :: 0 <= i < |ps| ==> ps[i].header_1.proposer_index == ps[i].header_2.proposer_index 
-//         requires forall i :: 0 <= i < |ps| ==> ps[i].header_1 == ps[i].header_2
-//         requires forall i :: 0 <= i < |ps| ==> ps[i].header_1.proposer_index as int < |s.validators| 
-//         requires forall i :: 0 <= i < |ps| ==> !s.validators[ps[i].header_1.proposer_index].slashed 
-//         requires forall i :: 0 <= i < |ps| ==> s.validators[ps[i].header_1.proposer_index].activation_epoch <= get_current_epoch(s) < s.validators[ps[i].header_1.proposer_index].withdrawable_epoch
-
-//         ensures forall i,j :: 0 <= i < j < |ps[..|ps|-1]| && i != j ==> ps[i].header_1.proposer_index!= ps[j].header_1.proposer_index
-//         ensures forall i :: 0 <= i < |ps[..|ps|-1]| ==> ps[i].header_1.slot == ps[i].header_2.slot;
-//         ensures forall i :: 0 <= i < |ps[..|ps|-1]| ==> ps[i].header_1.proposer_index == ps[i].header_2.proposer_index ;
-//         ensures forall i :: 0 <= i < |ps[..|ps|-1]| ==> ps[i].header_1 == ps[i].header_2;
-//         ensures forall i :: 0 <= i < |ps[..|ps|-1]| ==> ps[i].header_1.proposer_index as int < |s.validators| ;
-//         ensures forall i :: 0 <= i < |ps[..|ps|-1]| ==> !s.validators[ps[i].header_1.proposer_index].slashed ;
-//         ensures forall i :: 0 <= i < |ps[..|ps|-1]| ==> s.validators[ps[i].header_1.proposer_index].activation_epoch <= get_current_epoch(s) < s.validators[ps[i].header_1.proposer_index].withdrawable_epoch;
-           
-//     {
-//     }
-
-//     lemma helperPSLemma6(ps : seq<ProposerSlashing>)
-//         requires |ps| > 0
-//         ensures get_PS_validator_indices(ps[..|ps|-1]) + [ps[|ps|-1].header_1.proposer_index as int] == get_PS_validator_indices(ps)
-//         ensures forall i : int :: i !in get_PS_validator_indices(ps[..|ps|-1]) && i != ps[|ps|-1].header_1.proposer_index as int ==>
-//                 i !in get_PS_validator_indices(ps)
-//     {
-//         mappingPSIndices(ps);
-//         subsetMappingPSIndices(ps, |ps|-1);
-//     }
-
-
-//     ///////////////
-
-//     lemma AttestationHelperLemma(s: BeaconState, s1: BeaconState, a: Attestation)
-//         requires attestationIsWellFormed(s, a);
-//         requires s1.validators == s.validators
-//         requires s1.slot == s.slot
-//         requires s1.current_justified_checkpoint == s.current_justified_checkpoint
-//         requires s1.previous_justified_checkpoint == s.previous_justified_checkpoint
-//         ensures attestationIsWellFormed(s1, a);
-//     { // Thanks Dafny
-//     }
-
-//     //////////////////
-
-//     lemma VolExitLemma1(s: BeaconState, voluntary_exit: VoluntaryExit)
-//         requires |s.validators| == |s.balances|
-//         requires voluntary_exit.validator_index as int < |s.validators| 
-//         requires minimumActiveValidators(s)
-        
-//         requires !s.validators[voluntary_exit.validator_index].slashed
-//         requires s.validators[voluntary_exit.validator_index].activation_epoch <= get_current_epoch(s) < s.validators[voluntary_exit.validator_index].withdrawable_epoch
-
-//         requires s.validators[voluntary_exit.validator_index].exitEpoch == FAR_FUTURE_EPOCH
-//         requires get_current_epoch(s) >= voluntary_exit.epoch
-//         requires get_current_epoch(s) >= s.validators[voluntary_exit.validator_index].activation_epoch + SHARD_COMMITTEE_PERIOD 
-
-//         ensures minimumActiveValidators(updateVoluntaryExit(s, voluntary_exit))
-//     {
-//         // var s1 := updateVoluntaryExit(s, voluntary_exit);
-//         // assert get_current_epoch(s) == get_current_epoch(s1);
-//         // assert exists v :: 0 <= v < |s.validators| && s.validators[v].activation_epoch <= get_current_epoch(s) < s.validators[v].exitEpoch;
-//         // assert forall v :: 0 <= v < |s.validators| ==> s.validators[v].activation_epoch <= get_current_epoch(s) < s.validators[v].exitEpoch
-//         //                                             ==> s1.validators[v].activation_epoch <= get_current_epoch(s1) < s1.validators[v].exitEpoch;
-//         // assert exists v :: 0 <= v < |s1.validators| && s1.validators[v].activation_epoch <= get_current_epoch(s1) < s1.validators[v].exitEpoch;
-//         // assert exists v :: 0 <= v < |s1.validators| && is_active_validator(s1.validators[v], get_current_epoch(s1));
-//         // assert |get_active_validator_indices(s1.validators, get_current_epoch(s1))| > 0 ==> 
-//         //     (exists v :: 0 <= v < |s1.validators| && is_active_validator(s1.validators[v], get_current_epoch(s1)));
-//         // assert  minimumActiveValidators(s1);
-//     }
-
-
-//     lemma helperVoluntaryExitLemma3(s: BeaconState, ve: seq<VoluntaryExit>)
-//         requires forall i :: 0 <= i < |ve| ==> ve[i].validator_index as int < |s.validators| 
-//         //requires forall i :: 0 <= i < |ve| ==> is_active_validator(s.validators[ve[i].validator_index], get_current_epoch(s))
-//         requires forall i :: 0 <= i < |ve| ==> !s.validators[ve[i].validator_index].slashed
-//         requires forall i :: 0 <= i < |ve| ==> s.validators[ve[i].validator_index].activation_epoch <= get_current_epoch(s) < s.validators[ve[i].validator_index].withdrawable_epoch
-
-//         requires forall i :: 0 <= i < |ve| ==> s.validators[ve[i].validator_index].exitEpoch == FAR_FUTURE_EPOCH
-//         requires forall i :: 0 <= i < |ve| ==> get_current_epoch(s) >= s.validators[ve[i].validator_index].activation_epoch + SHARD_COMMITTEE_PERIOD 
-
-//         ensures forall i :: i in get_VolExit_validator_indices(ve) ==> 0 <= i < |s.validators| 
-        
-//         //ensures forall i :: i in get_VolExit_validator_indices(ve) ==> is_active_validator(s.validators[i], get_current_epoch(s))
-//         ensures forall i :: i in get_VolExit_validator_indices(ve) ==> !s.validators[i].slashed
-//         ensures forall i :: i in get_VolExit_validator_indices(ve) ==> s.validators[i].activation_epoch <= get_current_epoch(s) < s.validators[i].withdrawable_epoch
-
-//         ensures forall i :: i in get_VolExit_validator_indices(ve) ==> s.validators[i].exitEpoch == FAR_FUTURE_EPOCH
-//         ensures forall i :: i in get_VolExit_validator_indices(ve) ==> get_current_epoch(s) >= s.validators[i].activation_epoch + SHARD_COMMITTEE_PERIOD 
-//     {
-//         // Thanks Dafny
-//     }
-
-//     lemma helperVoluntaryExitLemma2(s: BeaconState, ve: seq<VoluntaryExit>)
-//         requires  |get_VolExit_validator_indices(ve)| > 0
-//         requires forall i :: i in get_VolExit_validator_indices(ve) ==> 0 <= i < |s.validators| 
-//         requires forall i :: i in get_VolExit_validator_indices(ve) ==> !s.validators[i].slashed
-//         requires forall i :: i in get_VolExit_validator_indices(ve) ==> s.validators[i].activation_epoch <= get_current_epoch(s) < s.validators[i].withdrawable_epoch
-//         requires forall i :: i in get_VolExit_validator_indices(ve) ==> s.validators[i].exitEpoch == FAR_FUTURE_EPOCH
-//         requires forall i :: i in get_VolExit_validator_indices(ve) ==> get_current_epoch(s) >= s.validators[i].activation_epoch + SHARD_COMMITTEE_PERIOD 
+        s.(
+            eth1_deposit_index := (s.eth1_deposit_index as int + 1) as uint64,
+            validators := if k in pk then 
+                                s.validators // unchanged validator members
+                            else 
+                                validator_append(s.validators, get_validator_from_deposit(d)), 
+            balances := if k in pk then 
+                            individualBalanceBoundMaintained(s.balances,d);
+                            updateExistingBalance(s, get_validator_index(pk, k), d.data.amount);
+                            increase_balance(s,get_validator_index(pk, k),d.data.amount).balances
+                        else 
+                            distBalancesProp(s.balances,[d.data.amount]);
+                            balance_append(s.balances, d.data.amount) 
+        )
+    }
     
-
-//         ensures forall i :: i in get_VolExit_validator_indices(ve[..|ve|-1]) ==> 0 <= i < |s.validators|
-//         ensures forall i :: i in get_VolExit_validator_indices(ve[..|ve|-1]) ==> !s.validators[i].slashed
-//         ensures forall i :: i in get_VolExit_validator_indices(ve[..|ve|-1]) ==> s.validators[i].activation_epoch <= get_current_epoch(s) < s.validators[i].withdrawable_epoch
-//         ensures forall i :: i in get_VolExit_validator_indices(ve[..|ve|-1]) ==> s.validators[i].exitEpoch == FAR_FUTURE_EPOCH
-//         ensures forall i :: i in get_VolExit_validator_indices(ve[..|ve|-1]) ==> get_current_epoch(s) >= s.validators[i].activation_epoch + SHARD_COMMITTEE_PERIOD
-//     {
-//         mappingVolExitIndices(ve);
-//         assert forall i :: 0 <= i < |ve| ==> get_VolExit_validator_indices(ve)[i] == ve[i].validator_index as int;
-
-//         subsetMappingVolExitIndices(ve, |ve|-1);
-//         assert get_VolExit_validator_indices(ve[..|ve|-1]) == get_VolExit_validator_indices(ve)[..|ve|-1];
+    /**
+     *  Take into account deposits in a block.
+     *
+     *  @param  s           A beacon state.
+     *  @param  deposits    A list of deposits from a block body.
+     *  @returns            The state obtained after taking account the deposits in `body` 
+     *                      from state `s` 
+     *
+     *  @note               The processing of deposits doesn't not use assume statements
+     *                      to prevent the overflow of amounts. The strategy of assuming
+     *                      that such overflow is not possible due to an upper limit on
+     *                      the amount of eth is used here and could be applied in other
+     *                      parts of the model where such assume statements are used.
+     */
+    function updateDeposits(s: BeaconState, deposits: seq<Deposit>) : BeaconState 
+        requires minimumActiveValidators(s)
+        requires s.eth1_deposit_index as int +  |deposits| < 0x10000000000000000 
+        requires |s.validators| == |s.balances|
+        requires |s.validators| + |deposits| <= VALIDATOR_REGISTRY_LIMIT as int
+        requires total_balances(s.balances) + total_deposits(deposits) < 0x10000000000000000 
+        // i.e. assume that (total balances + total deposits) isless than total eth
         
-//         assert forall i :: i in get_VolExit_validator_indices(ve) ==> 0 <= i < |s.validators|; // from requires
-//         assert forall i :: 0 <= i < |ve| ==> get_VolExit_validator_indices(ve)[i] == ve[i].validator_index as int;
-//         assert forall i :: 0 <= i < |ve| ==> ve[i].validator_index as int in get_VolExit_validator_indices(ve) ;
+        ensures updateDeposits(s, deposits).eth1_deposit_index 
+                == s.eth1_deposit_index  + |deposits| as uint64 
+        ensures |s.validators| 
+                <= |updateDeposits(s,deposits).validators| 
+                <= |s.validators| + |deposits| 
+        ensures total_balances(updateDeposits(s,deposits).balances) 
+                == total_balances(s.balances) + total_deposits(deposits)
+        ensures get_current_epoch(updateDeposits(s, deposits)) 
+                == get_current_epoch(s)
+        ensures minimumActiveValidators(updateDeposits(s, deposits))
         
-//     }
+        decreases |deposits|
+    {
+        if |deposits| == 0 then s
+        else 
+            updateDeposit(updateDeposits(s,deposits[..|deposits|-1]),deposits[|deposits|-1])
+    }
 
-//     lemma helperVoluntaryExitLemma(s: BeaconState, exit: VoluntaryExit)
-//         requires |s.validators| == |s.balances|
-//         requires exit.validator_index as int < |s.validators| 
-//         // requires is_active_validator(s.validators[voluntary_exit.validator_index], get_current_epoch(s))
-//         // (!v.slashed) && (v.activation_epoch <= epoch < v.withdrawable_epoch)
-//         requires !s.validators[exit.validator_index].slashed
-//         requires s.validators[exit.validator_index].activation_epoch <= get_current_epoch(s) < s.validators[exit.validator_index].withdrawable_epoch
-
-//         requires s.validators[exit.validator_index].exitEpoch == FAR_FUTURE_EPOCH
-//         requires get_current_epoch(s) >= exit.epoch
-//         requires get_current_epoch(s) >= s.validators[exit.validator_index].activation_epoch + SHARD_COMMITTEE_PERIOD 
-        
-//         ensures forall i :: 0 <= i < |s.validators| && i != exit.validator_index as int ==> updateVoluntaryExit(s, exit).validators[i].exitEpoch == s.validators[i].exitEpoch
-//         ensures forall i :: 0 <= i < |s.validators| && i != exit.validator_index as int ==> updateVoluntaryExit(s, exit).validators[i].slashed == s.validators[i].slashed
-//         ensures forall i :: 0 <= i < |s.validators| && i != exit.validator_index as int ==> updateVoluntaryExit(s, exit).validators[i].withdrawable_epoch == s.validators[i].withdrawable_epoch
-//     {
-//         // Thanks Dafny
-//     }
-
-//     lemma mappingVolExitIndices(ve: seq<VoluntaryExit>)
-//         ensures forall i :: 0 <= i < |ve| ==> get_VolExit_validator_indices(ve)[i] == ve[i].validator_index as int
-//     {
-//         //Thanks Dafny
-//     }
-
-//     lemma subsetMappingVolExitIndices(ve: seq<VoluntaryExit>, i : nat)
-//         requires 0 <= i < |ve|
-//         ensures get_VolExit_validator_indices(ve[..i]) == get_VolExit_validator_indices(ve)[..i]
-//     {
-//         if |ve| == 0 {}
-//         else {
-//             assert ve == ve[..i] + ve[i..];
-            
-//             mappingVolExitIndices(ve[..i]);
-//             assert forall j :: 0 <= j < |ve[..i]| ==> get_VolExit_validator_indices(ve[..i])[j] == ve[j].validator_index as int;
-
-//             mappingVolExitIndices(ve);
-//             assert forall j :: 0 <= j < |ve| ==> get_VolExit_validator_indices(ve)[j] == ve[j].validator_index as int;
-//         }
-//     }
-
-//     //lemma PSpreconditionLemma()
-//     lemma helperVolExitLemma4(ve : seq<VoluntaryExit>)
-//         requires |ve| > 0
-//         requires forall i,j :: 0 <= i < j < |ve| && i != j ==> ve[i].validator_index!= ve[j].validator_index // ve indices are unique
-//         ensures ve[|ve|-1].validator_index as int !in get_VolExit_validator_indices(ve[..|ve|-1])
-//     {
-//         mappingVolExitIndices(ve[..|ve|-1]);
-//         assert forall i :: 0 <= i < |ve[..|ve|-1]| ==> get_VolExit_validator_indices(ve[..|ve|-1])[i] == ve[i].validator_index as int;
-//     }
-
+    /**
+     *  The functional equivalent of process_voluntary_exit.
+     *  
+     *  @param  s       A beacon state.
+     *  @param  ve      A voluntary exit. 
+     *  @returns        A new state obtained from processing a voluntary exit.        
+     */
+    function updateVoluntaryExit(s: BeaconState, ve: VoluntaryExit) : BeaconState
+        requires minimumActiveValidators(s)
+        requires |s.validators| == |s.balances|
+        requires ve.validator_index as int < |s.validators| 
+        requires !s.validators[ve.validator_index].slashed
+        requires s.validators[ve.validator_index].activation_epoch 
+                <= get_current_epoch(s) 
+                < s.validators[ve.validator_index].withdrawable_epoch
+        requires s.validators[ve.validator_index].exitEpoch == FAR_FUTURE_EPOCH
+        requires get_current_epoch(s) >= ve.epoch
+        requires get_current_epoch(s) 
+                >= s.validators[ve.validator_index].activation_epoch + SHARD_COMMITTEE_PERIOD 
+         
+        ensures |updateVoluntaryExit(s, ve).validators| == |s.validators| 
+        ensures |updateVoluntaryExit(s, ve).validators| == |s.balances| 
+        ensures forall i :: 0 <= i < |s.validators| && i != ve.validator_index as int 
+                ==> updateVoluntaryExit(s, ve).validators[i] == s.validators[i]
+        ensures updateVoluntaryExit(s, ve) == initiate_validator_exit(s, ve.validator_index)
+        ensures get_current_epoch(updateVoluntaryExit(s, ve)) == get_current_epoch(s)
+        ensures get_current_epoch(s) 
+                >= updateVoluntaryExit(s, ve).validators[ve.validator_index].activation_epoch 
+                    + SHARD_COMMITTEE_PERIOD 
+        ensures forall i :: 0 <= i < |s.validators| 
+                ==> updateVoluntaryExit(s, ve).validators[i].activation_epoch 
+                    == s.validators[i].activation_epoch
+        ensures minimumActiveValidators(updateVoluntaryExit(s, ve))
+    {
+        var s' := initiate_validator_exit(s, ve.validator_index);
+        assert minimumActiveValidators(s');
+        s'
+    }
     
-
-
+    /**
+     *  The functional equivalent of processing a sequence of voluntary exits.
+     *  
+     *  @param  s       A beacon state.
+     *  @param  ve      A sequence of voluntary exits. 
+     *  @returns        A new state obtained from processing ve.        
+     */
+    function updateVoluntaryExits(s: BeaconState, ve: seq<VoluntaryExit>) : BeaconState
+        requires minimumActiveValidators(s)
+        requires forall i,j :: 0 <= i < j < |ve| && i != j 
+                ==> ve[i].validator_index != ve[j].validator_index // ve indices are unique
+        requires |s.validators| == |s.balances|
+        requires forall i :: 0 <= i < |ve| ==> get_current_epoch(s) >= ve[i].epoch
+        requires forall i :: 0 <= i < |ve| ==> ve[i].validator_index as int < |s.validators| 
+        requires forall i :: 0 <= i < |ve| ==> !s.validators[ve[i].validator_index].slashed
+        requires forall i :: 0 <= i < |ve| ==> s.validators[ve[i].validator_index].activation_epoch 
+                                                <= get_current_epoch(s) 
+                                                < s.validators[ve[i].validator_index].withdrawable_epoch
+        requires forall i :: 0 <= i < |ve| 
+                ==> s.validators[ve[i].validator_index].exitEpoch == FAR_FUTURE_EPOCH
+        requires forall i :: 0 <= i < |ve| 
+                ==> s.validators[ve[i].validator_index].activation_epoch as nat + SHARD_COMMITTEE_PERIOD as nat 
+                    <= get_current_epoch(s) as nat < 0x10000000000000000 
    
-    
+        ensures |updateVoluntaryExits(s, ve).validators| == |s.validators|
+        ensures |updateVoluntaryExits(s, ve).validators| == |updateVoluntaryExits(s, ve).balances|
+        ensures updateVoluntaryExits(s, ve).slot == s.slot
+        ensures get_current_epoch(updateVoluntaryExits(s, ve)) == get_current_epoch(s)
+        ensures forall i :: 0 <= i < |s.validators| 
+                ==> updateVoluntaryExits(s, ve).validators[i].activation_epoch == s.validators[i].activation_epoch
+        ensures forall i :: 0 <= i < |s.validators| && i !in get_VolExit_validator_indices(ve) 
+                ==> updateVoluntaryExits(s, ve).validators[i] == s.validators[i]
+        ensures minimumActiveValidators(updateVoluntaryExits(s, ve))
+        
+        decreases |ve|
+    {
+        if |ve| == 0 then 
+            s
+        else
+            var s1 := updateVoluntaryExits(s,ve[..|ve|-1]);
 
-    
-    
+            assert ve[|ve|-1] !in ve[..|ve|-1] ;
+            assert minimumActiveValidators(s1);
+            assert |s1.validators| == |s1.balances| == |s.validators|;
+            assert ve[|ve|-1].validator_index as int < |s.validators|; 
+            
+            VEHelperLemma1(s, s1,  ve[..|ve|-1], ve[|ve|-1], ve);
+            assert s1.validators[ve[|ve|-1].validator_index] == s.validators[ve[|ve|-1].validator_index];
+            assert !s1.validators[ve[|ve|-1].validator_index].slashed;
+            assert s1.validators[ve[|ve|-1].validator_index].activation_epoch 
+                    <= get_current_epoch(s) 
+                    < s1.validators[ve[|ve|-1].validator_index].withdrawable_epoch;
+            assert s1.validators[ve[|ve|-1].validator_index].exitEpoch == FAR_FUTURE_EPOCH;
+            assert get_current_epoch(s) >= ve[|ve|-1].epoch;
+            assert get_current_epoch(s) 
+                    >= s1.validators[ve[|ve|-1].validator_index].activation_epoch + SHARD_COMMITTEE_PERIOD ;
 
+            var s2 := updateVoluntaryExit(s1, ve[|ve|-1]);
+
+            assert |s2.validators| == |s.validators|;
+            assert |s2.validators| == |s2.balances|;
+            assert s2.slot == s.slot;
+            assert get_current_epoch(s2) == get_current_epoch(s);
+            assert forall i :: 0 <= i < |s.validators| 
+                ==> s2.validators[i].activation_epoch == s.validators[i].activation_epoch;
+            
+            VEHelperLemma2(s, s2,  ve[..|ve|-1], ve[|ve|-1], ve);
+            assert forall i :: 0 <= i < |s.validators| && i !in get_VolExit_validator_indices(ve) 
+                ==> s2.validators[i] == s.validators[i];
+            assert minimumActiveValidators(s2);
+
+            s2
+
+    }
+    
 }
