src/dafny/beacon/statetransition/ProcessOperations.p.dfy
@@ -25,7 +25,6 @@ include "../attestations/AttestationsTypes.dfy"
 include "../attestations/AttestationsHelpers.dfy"
 include "../Helpers.dfy"
 include "../Helpers.s.dfy"
-//include "ProcessOperations.dfy"
 
 /**
  *  Proofs for process operations
@@ -45,8 +44,7 @@ module ProcessOperationsProofs {
     import opened BeaconHelperSpec
     import opened MathHelpers
     import opened SeqHelpers
-    //import ProcessOperations
-
+ 
     
     // Helper lemmas
 
@@ -100,43 +98,58 @@ module ProcessOperationsProofs {
         // Thanks Dafny
     }
 
+/////////////////////
 
+    lemma mappingPSIndices(ps: seq<ProposerSlashing>)
+        ensures forall i :: 0 <= i < |ps| ==> get_PS_validator_indices(ps)[i] == ps[i].header_1.proposer_index as int
+    {
+        //Thanks Dafny
+    }
 
-// lemma updateBalTotalBySingleDeposit(s: BeaconState, d: Deposit)
-//         requires s.eth1_deposit_index as int +  1 < 0x10000000000000000 
-//         requires |s.validators| == |s.balances|
-//         requires |s.validators| + 1 <= VALIDATOR_REGISTRY_LIMIT as int
-//         requires total_balances(s.balances) + d.data.amount as int < 0x10000000000000000
+    lemma subsetMappingPSIndices(ps: seq<ProposerSlashing>, i : nat)
+        requires 0 <= i < |ps|
+        ensures get_PS_validator_indices(ps[..i]) == get_PS_validator_indices(ps)[..i]
+    {
+        if |ps| == 0 {}
+        else {
+            assert ps == ps[..i] + ps[i..];
+            
+            mappingPSIndices(ps[..i]);
+            assert forall j :: 0 <= j < |ps[..i]| ==> get_PS_validator_indices(ps[..i])[j] == ps[j].header_1.proposer_index as int;
+
+            mappingPSIndices(ps);
+            assert forall j :: 0 <= j < |ps| ==> get_PS_validator_indices(ps)[j] == ps[j].header_1.proposer_index as int;
+        }
+    }
+
+    lemma PSHelperLemma1(s: BeaconState, s1: BeaconState, ps1: seq<ProposerSlashing>, ps2: ProposerSlashing, ps: seq<ProposerSlashing>)
+        requires |ps1| == |ps|-1
+        requires ps1 == ps[..|ps|-1]
+        requires ps2 == ps[|ps|-1]
+
+        //requires ps1 + [ps2] == ps
+        requires forall i,j :: 0 <= i < j < |ps| && i != j ==> ps[i].header_1.proposer_index!= ps[j].header_1.proposer_index 
+        requires forall i :: 0 <= i < |ps1| ==> ps1[i].header_1.proposer_index as int < |s.validators| 
+        requires ps2.header_1.proposer_index as int < |s.validators| 
+        requires |s1.validators| == |s.validators|
+
+        requires forall i :: 0 <= i < |s.validators| && i !in get_PS_validator_indices(ps1) ==> s1.validators[i] == s.validators[i]
+        requires ps2 !in ps1
+
+        ensures s1.validators[ps2.header_1.proposer_index] == s.validators[ps2.header_1.proposer_index]
+    {
+        seqInitLast<ProposerSlashing>(ps, |ps|-1);
+        assert ps[..|ps|-1] + [ps[|ps|-1]] == ps[..|ps|];
+        assert ps[..|ps|] == ps;
+        assert ps1 + [ps2] == ps;
         
-//         ensures total_balances(updateDeposit(s,d).balances) == total_balances(s.balances) + d.data.amount as int < 0x10000000000000000
-//         //ensures total_balances(updateDeposit(s,d).balances) == total_balances(s.balances) + total_deposits([d]) 
-//     {
-//         var pk := seqKeysInValidators(s.validators); 
-//         if |s.balances| == 0 {
-//             // Thanks Dafny
-//         }
-//         else {
-//             if d.data.pubkey in pk {
-//                 var index := get_validator_index(pk, d.data.pubkey);
-//                 individualBalanceBoundMaintained(s.balances,d);
-//                 //assert updateDeposit(s,d).balances ==  increase_balance(s,index,d.data.amount).balances;
-//                 //assert increase_balance(s,index,d.data.amount).balances[index] == s.balances[index] + d.data.amount;
-//                 //assert forall i :: 0 <= i < |s.balances| && i != index as int ==> increase_balance(s,index,d.data.amount).balances[i] == s.balances[i];
-//                 //assert total_balances(updateDeposit(s,d).balances) == total_balances(increase_balance(s,index,d.data.amount).balances) ;
-//                 updateExistingBalance(s, index, d.data.amount);
-//                 //assert total_balances(updateDeposit(s,d).balances) == total_balances(s.balances) + d.data.amount as int ;
-//             }
-//             else {
-//                 //assert updateDeposit(s,d).balances == s.balances + [d.data.amount];
-//                 distBalancesProp(s.balances,[d.data.amount]);
-//                 //assert total_balances(s.balances + [d.data.amount]) == total_balances(s.balances) + total_balances([d.data.amount]);
-//             }
-//         }
-//     }
+        mappingPSIndices(ps1);
+        assert forall i :: 0 <= i < |ps1| ==> get_PS_validator_indices(ps1)[i] == ps1[i].header_1.proposer_index as int;
+        assert forall i :: 0 <= i < |ps[..|ps|-1]|  ==> ps[i].header_1.proposer_index != ps[|ps|-1].header_1.proposer_index ;
+        assert ps2.header_1.proposer_index as int !in get_PS_validator_indices(ps1);
+    }
 
-
-///////////////////////////
-    lemma testLemma3(s: BeaconState, s2: BeaconState, ps1: seq<ProposerSlashing>, ps2: ProposerSlashing, ps: seq<ProposerSlashing>)
+    lemma PSHelperLemma2(s: BeaconState, s2: BeaconState, ps1: seq<ProposerSlashing>, ps2: ProposerSlashing, ps: seq<ProposerSlashing>)
         requires |ps1| == |ps|-1
         requires ps1 == ps[..|ps|-1]
         requires ps2 == ps[|ps|-1]
@@ -172,281 +185,69 @@ module ProcessOperationsProofs {
     }
 
 
+    lemma VEHelperLemma1(s: BeaconState, s1: BeaconState, ve1: seq<VoluntaryExit>, ve2: VoluntaryExit, ve: seq<VoluntaryExit>)
+        requires |ve1| == |ve|-1
+        requires ve1 == ve[..|ve|-1]
+        requires ve2 == ve[|ve|-1]
 
-
-    lemma testLemma1(s: BeaconState, s1: BeaconState, ps1: seq<ProposerSlashing>, ps2: ProposerSlashing, ps: seq<ProposerSlashing>)
-        requires |ps1| == |ps|-1
-        requires ps1 == ps[..|ps|-1]
-        requires ps2 == ps[|ps|-1]
-
-        //requires ps1 + [ps2] == ps
-        requires forall i,j :: 0 <= i < j < |ps| && i != j ==> ps[i].header_1.proposer_index!= ps[j].header_1.proposer_index 
-        requires forall i :: 0 <= i < |ps1| ==> ps1[i].header_1.proposer_index as int < |s.validators| 
-        requires ps2.header_1.proposer_index as int < |s.validators| 
+        //requires ve1 + [ve2] == ve
+        requires forall i,j :: 0 <= i < j < |ve| && i != j ==> ve[i].validator_index!= ve[j].validator_index 
+        requires forall i :: 0 <= i < |ve1| ==> ve1[i].validator_index as int < |s.validators| 
+        requires ve2.validator_index as int < |s.validators| 
         requires |s1.validators| == |s.validators|
 
-        requires forall i :: 0 <= i < |s.validators| && i !in get_PS_validator_indices(ps1) ==> s1.validators[i] == s.validators[i]
-        requires ps2 !in ps1
+        requires forall i :: 0 <= i < |s.validators| && i !in get_VolExit_validator_indices(ve1) ==> s1.validators[i] == s.validators[i]
+        requires ve2 !in ve1
 
-        ensures s1.validators[ps2.header_1.proposer_index] == s.validators[ps2.header_1.proposer_index]
+        ensures s1.validators[ve2.validator_index] == s.validators[ve2.validator_index]
     {
-        seqInitLast<ProposerSlashing>(ps, |ps|-1);
-        assert ps[..|ps|-1] + [ps[|ps|-1]] == ps[..|ps|];
-        assert ps[..|ps|] == ps;
-        assert ps1 + [ps2] == ps;
+        seqInitLast<VoluntaryExit>(ve, |ve|-1);
+        assert ve[..|ve|-1] + [ve[|ve|-1]] == ve[..|ve|];
+        assert ve[..|ve|] == ve;
+        assert ve1 + [ve2] == ve;
         
-        mappingPSIndices(ps1);
-        assert forall i :: 0 <= i < |ps1| ==> get_PS_validator_indices(ps1)[i] == ps1[i].header_1.proposer_index as int;
-        assert forall i :: 0 <= i < |ps[..|ps|-1]|  ==> ps[i].header_1.proposer_index != ps[|ps|-1].header_1.proposer_index ;
-        assert ps2.header_1.proposer_index as int !in get_PS_validator_indices(ps1);
+        mappingVolExitIndices(ve1);
+        assert forall i :: 0 <= i < |ve1| ==> get_VolExit_validator_indices(ve1)[i] == ve1[i].validator_index as int;
+        assert forall i :: 0 <= i < |ve[..|ve|-1]|  ==> ve[i].validator_index != ve[|ve|-1].validator_index ;
+        assert ve2.validator_index as int !in get_VolExit_validator_indices(ve1);
     }
 
+    lemma VEHelperLemma2(s: BeaconState, s1: BeaconState, ve1: seq<VoluntaryExit>, ve2: VoluntaryExit, ve: seq<VoluntaryExit>)
+        requires |ve1| == |ve|-1
+        requires ve1 == ve[..|ve|-1]
+        requires ve2 == ve[|ve|-1]
 
+        //requires ve1 + [ve2] == ve
+        requires forall i,j :: 0 <= i < j < |ve| && i != j ==> ve[i].validator_index!= ve[j].validator_index 
+        requires forall i :: 0 <= i < |ve1| ==> ve1[i].validator_index as int < |s.validators| 
+        requires ve2.validator_index as int < |s.validators| 
+        requires |s1.validators| == |s.validators|
 
-    lemma mappingPSIndices(ps: seq<ProposerSlashing>)
-        ensures forall i :: 0 <= i < |ps| ==> get_PS_validator_indices(ps)[i] == ps[i].header_1.proposer_index as int
+        requires forall i :: 0 <= i < |s.validators| && i !in (get_VolExit_validator_indices(ve1) + [ve2.validator_index as int]) 
+                ==> s1.validators[i] == s.validators[i]
+        
+        ensures forall i :: 0 <= i < |s.validators| && i !in get_VolExit_validator_indices(ve) ==> s1.validators[i] == s.validators[i]
     {
-        //Thanks Dafny
-    }
-
-    lemma subsetMappingPSIndices(ps: seq<ProposerSlashing>, i : nat)
-        requires 0 <= i < |ps|
-        ensures get_PS_validator_indices(ps[..i]) == get_PS_validator_indices(ps)[..i]
-    {
-        if |ps| == 0 {}
-        else {
-            assert ps == ps[..i] + ps[i..];
-            
-            mappingPSIndices(ps[..i]);
-            assert forall j :: 0 <= j < |ps[..i]| ==> get_PS_validator_indices(ps[..i])[j] == ps[j].header_1.proposer_index as int;
-
-            mappingPSIndices(ps);
-            assert forall j :: 0 <= j < |ps| ==> get_PS_validator_indices(ps)[j] == ps[j].header_1.proposer_index as int;
-        }
-    }
-
-    // lemma helperPSLemma(s: BeaconState, ps: ProposerSlashing)
-    //     requires ps.header_1.slot == ps.header_2.slot
-    //     requires ps.header_1.proposer_index == ps.header_2.proposer_index 
-    //     requires ps.header_1 == ps.header_2
-    //     requires ps.header_1.proposer_index as int < |s.validators| 
-
-    //     // requires is_active_validator: (!v.slashed) && (v.activation_epoch <= epoch < v.withdrawable_epoch)
-    //     requires !s.validators[ps.header_1.proposer_index].slashed
-    //     requires s.validators[ps.header_1.proposer_index].activation_epoch <= get_current_epoch(s) < s.validators[ps.header_1.proposer_index].withdrawable_epoch
- 
-    //     requires |get_active_validator_indices(s.validators, get_current_epoch(s))| > 0
-    //     requires |s.validators| == |s.balances|
+        seqInitLast<VoluntaryExit>(ve, |ve|-1);
+        assert ve[..|ve|-1] + [ve[|ve|-1]] == ve[..|ve|];
+        assert ve[..|ve|] == ve;
+        assert ve1 + [ve2] == ve;
         
-    //     ensures forall i :: 0 <= i < |s.validators| && i != ps.header_1.proposer_index as int ==> updateProposerSlashing(s, ps).validators[i].exitEpoch == s.validators[i].exitEpoch
-    //     ensures forall i :: 0 <= i < |s.validators| && i != ps.header_1.proposer_index as int ==> updateProposerSlashing(s, ps).validators[i].slashed == s.validators[i].slashed
-    //     ensures forall i :: 0 <= i < |s.validators| && i != ps.header_1.proposer_index as int ==> updateProposerSlashing(s, ps).validators[i].withdrawable_epoch == s.validators[i].withdrawable_epoch
-    // {
-    //     // Thanks Dafny
-    //}
+        subsetMappingVolExitIndices(ve,|ve|-1);
+        assert ve1 == ve[..|ve|-1];
+        assert get_VolExit_validator_indices(ve[..|ve|-1]) == get_VolExit_validator_indices(ve1) == get_VolExit_validator_indices(ve)[..|ve|-1];
 
-    // lemma helperPSLemma2(s: BeaconState, ps: seq<ProposerSlashing>)
-    //     requires  |get_PS_validator_indices(ps)| > 0
-    //     requires forall i :: i in get_PS_validator_indices(ps) ==> 0 <= i < |s.validators| 
-    //     requires forall i :: i in get_PS_validator_indices(ps) ==> !s.validators[i].slashed
-    //     requires forall i :: i in get_PS_validator_indices(ps) ==> s.validators[i].activation_epoch <= get_current_epoch(s) < s.validators[i].withdrawable_epoch
-        
-
-    //     ensures forall i :: i in get_PS_validator_indices(ps[..|ps|-1]) ==> 0 <= i < |s.validators|
-    //     ensures forall i :: i in get_PS_validator_indices(ps[..|ps|-1]) ==> !s.validators[i].slashed
-    //     ensures forall i :: i in get_PS_validator_indices(ps[..|ps|-1]) ==> s.validators[i].activation_epoch <= get_current_epoch(s) < s.validators[i].withdrawable_epoch
-    // {
-    //     mappingPSIndices(ps);
-    //     assert forall i :: 0 <= i < |ps| ==> get_PS_validator_indices(ps)[i] == ps[i].header_1.proposer_index as int;
-
-    //     subsetMappingPSIndices(ps, |ps|-1);
-    //     assert get_PS_validator_indices(ps[..|ps|-1]) == get_PS_validator_indices(ps)[..|ps|-1];
-        
-    //     assert forall i :: i in get_PS_validator_indices(ps) ==> 0 <= i < |s.validators|; // from requires
-    //     assert forall i :: 0 <= i < |ps| ==> get_PS_validator_indices(ps)[i] == ps[i].header_1.proposer_index as int;
-    //     assert forall i :: 0 <= i < |ps| ==> ps[i].header_1.proposer_index as int in get_PS_validator_indices(ps) ;
-        
-    // }
-
-
-    // lemma updateProposerSlashingLemma(s: BeaconState, ps : ProposerSlashing)
-    //     requires ps.header_1.slot == ps.header_2.slot
-    //     requires ps.header_1.proposer_index == ps.header_2.proposer_index 
-    //     requires ps.header_1 == ps.header_2
-    //     requires ps.header_1.proposer_index as int < |s.validators| 
-    //     //requires is_slashable_validator(s.validators[ps.header_1.proposer_index], get_current_epoch(s));
-    //     //(!v.slashed) && (v.activation_epoch <= epoch < v.withdrawable_epoch)
-    //     requires !s.validators[ps.header_1.proposer_index].slashed
-    //     requires s.validators[ps.header_1.proposer_index].activation_epoch <= get_current_epoch(s) < s.validators[ps.header_1.proposer_index].withdrawable_epoch
-        
-    //     requires |get_active_validator_indices(s.validators, get_current_epoch(s))| > 0
-    //     requires |s.validators| == |s.balances|
-        
-    //     ensures |get_active_validator_indices(updateProposerSlashing(s, ps).validators, get_current_epoch(s))| > 0
-    // {
-    //     var index := ps.header_1.proposer_index; // validator to be slashed
-    //     var slashable_validator := s.validators[index];
-    //     var epoch : Epoch := get_current_epoch(s);
-
-    //     assert updateProposerSlashing(s, ps) == slash_validator(s, ps.header_1.proposer_index, get_beacon_proposer_index(s));
-    //     slashValidatorPreservesActivateValidators(s, ps.header_1.proposer_index, get_beacon_proposer_index(s));
-    //     assert |get_active_validator_indices(updateProposerSlashing(s, ps).validators, get_current_epoch(s))| > 0;
-
-    // }
-
-    // lemma helperPSLemma3(s: BeaconState, ps : seq<ProposerSlashing>)
-    //     requires forall i :: 0 <= i < |ps| ==> ps[i].header_1.proposer_index as int < |s.validators| 
-    //     requires forall i :: 0 <= i < |ps| ==> !s.validators[ps[i].header_1.proposer_index].slashed 
-    //     requires forall i :: 0 <= i < |ps| ==> s.validators[ps[i].header_1.proposer_index].activation_epoch <= get_current_epoch(s) < s.validators[ps[i].header_1.proposer_index].withdrawable_epoch
-
-    //     ensures forall i :: i in get_PS_validator_indices(ps) ==> 0 <= i < |s.validators|
-    //     ensures forall i :: i in get_PS_validator_indices(ps) ==> !s.validators[i].slashed
-    //     ensures forall i :: i in get_PS_validator_indices(ps) ==> s.validators[i].activation_epoch <= get_current_epoch(s) < s.validators[i].withdrawable_epoch
-    // {
-    //     // Thanks Dafny
-    // }
-
-    // lemma helperPSLemma4(ps : seq<ProposerSlashing>)
-    //     requires |ps| > 0
-    //     requires forall i,j :: 0 <= i < j < |ps| && i != j ==> ps[i].header_1.proposer_index!= ps[j].header_1.proposer_index // ve indices are unique
-    //     ensures ps[|ps|-1].header_1.proposer_index as int !in get_PS_validator_indices(ps[..|ps|-1])
-    // {
-    //     mappingPSIndices(ps[..|ps|-1]);
-    //     assert forall i :: 0 <= i < |ps[..|ps|-1]| ==> get_PS_validator_indices(ps[..|ps|-1])[i] == ps[i].header_1.proposer_index as int;
-    // }
-
-    // lemma helperPSLemma5(s: BeaconState, ps : seq<ProposerSlashing>)
-    //     requires |ps| > 0
-    //     requires forall i,j :: 0 <= i < j < |ps| && i != j ==> ps[i].header_1.proposer_index!= ps[j].header_1.proposer_index // ve indices are unique
-    //     requires forall i :: 0 <= i < |ps| ==> ps[i].header_1.slot == ps[i].header_2.slot
-    //     requires forall i :: 0 <= i < |ps| ==> ps[i].header_1.proposer_index == ps[i].header_2.proposer_index 
-    //     requires forall i :: 0 <= i < |ps| ==> ps[i].header_1 == ps[i].header_2
-    //     requires forall i :: 0 <= i < |ps| ==> ps[i].header_1.proposer_index as int < |s.validators| 
-    //     requires forall i :: 0 <= i < |ps| ==> !s.validators[ps[i].header_1.proposer_index].slashed 
-    //     requires forall i :: 0 <= i < |ps| ==> s.validators[ps[i].header_1.proposer_index].activation_epoch <= get_current_epoch(s) < s.validators[ps[i].header_1.proposer_index].withdrawable_epoch
-
-    //     ensures forall i,j :: 0 <= i < j < |ps[..|ps|-1]| && i != j ==> ps[i].header_1.proposer_index!= ps[j].header_1.proposer_index
-    //     ensures forall i :: 0 <= i < |ps[..|ps|-1]| ==> ps[i].header_1.slot == ps[i].header_2.slot;
-    //     ensures forall i :: 0 <= i < |ps[..|ps|-1]| ==> ps[i].header_1.proposer_index == ps[i].header_2.proposer_index ;
-    //     ensures forall i :: 0 <= i < |ps[..|ps|-1]| ==> ps[i].header_1 == ps[i].header_2;
-    //     ensures forall i :: 0 <= i < |ps[..|ps|-1]| ==> ps[i].header_1.proposer_index as int < |s.validators| ;
-    //     ensures forall i :: 0 <= i < |ps[..|ps|-1]| ==> !s.validators[ps[i].header_1.proposer_index].slashed ;
-    //     ensures forall i :: 0 <= i < |ps[..|ps|-1]| ==> s.validators[ps[i].header_1.proposer_index].activation_epoch <= get_current_epoch(s) < s.validators[ps[i].header_1.proposer_index].withdrawable_epoch;
-           
-    // {
-    // }
-
-    // lemma helperPSLemma6(ps : seq<ProposerSlashing>)
-    //     requires |ps| > 0
-    //     ensures get_PS_validator_indices(ps[..|ps|-1]) + [ps[|ps|-1].header_1.proposer_index as int] == get_PS_validator_indices(ps)
-    //     ensures forall i : int :: i !in get_PS_validator_indices(ps[..|ps|-1]) && i != ps[|ps|-1].header_1.proposer_index as int ==>
-    //             i !in get_PS_validator_indices(ps)
-    // {
-    //     mappingPSIndices(ps);
-    //     subsetMappingPSIndices(ps, |ps|-1);
-    // }
-
-
-    ///////////////
-
-    
-
-    //////////////////
-
-    // lemma VolExitLemma1(s: BeaconState, voluntary_exit: VoluntaryExit)
-    //     requires |s.validators| == |s.balances|
-    //     requires voluntary_exit.validator_index as int < |s.validators| 
-    //     requires minimumActiveValidators(s)
-        
-    //     requires !s.validators[voluntary_exit.validator_index].slashed
-    //     requires s.validators[voluntary_exit.validator_index].activation_epoch <= get_current_epoch(s) < s.validators[voluntary_exit.validator_index].withdrawable_epoch
-
-    //     requires s.validators[voluntary_exit.validator_index].exitEpoch == FAR_FUTURE_EPOCH
-    //     requires get_current_epoch(s) >= voluntary_exit.epoch
-    //     requires get_current_epoch(s) >= s.validators[voluntary_exit.validator_index].activation_epoch + SHARD_COMMITTEE_PERIOD 
-
-    //     ensures minimumActiveValidators(updateVoluntaryExit(s, voluntary_exit))
-    // {
-    //     // var s1 := updateVoluntaryExit(s, voluntary_exit);
-    //     // assert get_current_epoch(s) == get_current_epoch(s1);
-    //     // assert exists v :: 0 <= v < |s.validators| && s.validators[v].activation_epoch <= get_current_epoch(s) < s.validators[v].exitEpoch;
-    //     // assert forall v :: 0 <= v < |s.validators| ==> s.validators[v].activation_epoch <= get_current_epoch(s) < s.validators[v].exitEpoch
-    //     //                                             ==> s1.validators[v].activation_epoch <= get_current_epoch(s1) < s1.validators[v].exitEpoch;
-    //     // assert exists v :: 0 <= v < |s1.validators| && s1.validators[v].activation_epoch <= get_current_epoch(s1) < s1.validators[v].exitEpoch;
-    //     // assert exists v :: 0 <= v < |s1.validators| && is_active_validator(s1.validators[v], get_current_epoch(s1));
-    //     // assert |get_active_validator_indices(s1.validators, get_current_epoch(s1))| > 0 ==> 
-    //     //     (exists v :: 0 <= v < |s1.validators| && is_active_validator(s1.validators[v], get_current_epoch(s1)));
-    //     // assert  minimumActiveValidators(s1);
-    // }
-
-
-    lemma helperVoluntaryExitLemma3(s: BeaconState, ve: seq<VoluntaryExit>)
-        requires forall i :: 0 <= i < |ve| ==> ve[i].validator_index as int < |s.validators| 
-        //requires forall i :: 0 <= i < |ve| ==> is_active_validator(s.validators[ve[i].validator_index], get_current_epoch(s))
-        requires forall i :: 0 <= i < |ve| ==> !s.validators[ve[i].validator_index].slashed
-        requires forall i :: 0 <= i < |ve| ==> s.validators[ve[i].validator_index].activation_epoch <= get_current_epoch(s) < s.validators[ve[i].validator_index].withdrawable_epoch
-
-        requires forall i :: 0 <= i < |ve| ==> s.validators[ve[i].validator_index].exitEpoch == FAR_FUTURE_EPOCH
-        requires forall i :: 0 <= i < |ve| ==> get_current_epoch(s) >= s.validators[ve[i].validator_index].activation_epoch + SHARD_COMMITTEE_PERIOD 
-
-        ensures forall i :: i in get_VolExit_validator_indices(ve) ==> 0 <= i < |s.validators| 
-        
-        //ensures forall i :: i in get_VolExit_validator_indices(ve) ==> is_active_validator(s.validators[i], get_current_epoch(s))
-        ensures forall i :: i in get_VolExit_validator_indices(ve) ==> !s.validators[i].slashed
-        ensures forall i :: i in get_VolExit_validator_indices(ve) ==> s.validators[i].activation_epoch <= get_current_epoch(s) < s.validators[i].withdrawable_epoch
-
-        ensures forall i :: i in get_VolExit_validator_indices(ve) ==> s.validators[i].exitEpoch == FAR_FUTURE_EPOCH
-        ensures forall i :: i in get_VolExit_validator_indices(ve) ==> get_current_epoch(s) >= s.validators[i].activation_epoch + SHARD_COMMITTEE_PERIOD 
-    {
-        // Thanks Dafny
-    }
-
-    lemma helperVoluntaryExitLemma2(s: BeaconState, ve: seq<VoluntaryExit>)
-        requires  |get_VolExit_validator_indices(ve)| > 0
-        requires forall i :: i in get_VolExit_validator_indices(ve) ==> 0 <= i < |s.validators| 
-        requires forall i :: i in get_VolExit_validator_indices(ve) ==> !s.validators[i].slashed
-        requires forall i :: i in get_VolExit_validator_indices(ve) ==> s.validators[i].activation_epoch <= get_current_epoch(s) < s.validators[i].withdrawable_epoch
-        requires forall i :: i in get_VolExit_validator_indices(ve) ==> s.validators[i].exitEpoch == FAR_FUTURE_EPOCH
-        requires forall i :: i in get_VolExit_validator_indices(ve) ==> get_current_epoch(s) >= s.validators[i].activation_epoch + SHARD_COMMITTEE_PERIOD 
-    
-
-        ensures forall i :: i in get_VolExit_validator_indices(ve[..|ve|-1]) ==> 0 <= i < |s.validators|
-        ensures forall i :: i in get_VolExit_validator_indices(ve[..|ve|-1]) ==> !s.validators[i].slashed
-        ensures forall i :: i in get_VolExit_validator_indices(ve[..|ve|-1]) ==> s.validators[i].activation_epoch <= get_current_epoch(s) < s.validators[i].withdrawable_epoch
-        ensures forall i :: i in get_VolExit_validator_indices(ve[..|ve|-1]) ==> s.validators[i].exitEpoch == FAR_FUTURE_EPOCH
-        ensures forall i :: i in get_VolExit_validator_indices(ve[..|ve|-1]) ==> get_current_epoch(s) >= s.validators[i].activation_epoch + SHARD_COMMITTEE_PERIOD
-    {
+        ////////
         mappingVolExitIndices(ve);
         assert forall i :: 0 <= i < |ve| ==> get_VolExit_validator_indices(ve)[i] == ve[i].validator_index as int;
+        assert get_VolExit_validator_indices(ve)[|ve|-1] == ve[|ve|-1].validator_index as int == ve2.validator_index as int;
 
-        subsetMappingVolExitIndices(ve, |ve|-1);
-        assert get_VolExit_validator_indices(ve[..|ve|-1]) == get_VolExit_validator_indices(ve)[..|ve|-1];
-        
-        assert forall i :: i in get_VolExit_validator_indices(ve) ==> 0 <= i < |s.validators|; // from requires
-        assert forall i :: 0 <= i < |ve| ==> get_VolExit_validator_indices(ve)[i] == ve[i].validator_index as int;
-        assert forall i :: 0 <= i < |ve| ==> ve[i].validator_index as int in get_VolExit_validator_indices(ve) ;
-        
+        assert get_VolExit_validator_indices(ve)[..|ve|-1] + [get_VolExit_validator_indices(ve)[|ve|-1]] == get_VolExit_validator_indices(ve);
+    
+        assert get_VolExit_validator_indices(ve1) + [ve2.validator_index as int] == get_VolExit_validator_indices(ve);
+
     }
-
-    // lemma helperVoluntaryExitLemma(s: BeaconState, exit: VoluntaryExit)
-    //     requires |s.validators| == |s.balances|
-    //     requires exit.validator_index as int < |s.validators| 
-    //     // requires is_active_validator(s.validators[voluntary_exit.validator_index], get_current_epoch(s))
-    //     // (!v.slashed) && (v.activation_epoch <= epoch < v.withdrawable_epoch)
-    //     requires !s.validators[exit.validator_index].slashed
-    //     requires s.validators[exit.validator_index].activation_epoch <= get_current_epoch(s) < s.validators[exit.validator_index].withdrawable_epoch
-
-    //     requires s.validators[exit.validator_index].exitEpoch == FAR_FUTURE_EPOCH
-    //     requires get_current_epoch(s) >= exit.epoch
-    //     requires get_current_epoch(s) >= s.validators[exit.validator_index].activation_epoch + SHARD_COMMITTEE_PERIOD 
-        
-    //     ensures forall i :: 0 <= i < |s.validators| && i != exit.validator_index as int ==> updateVoluntaryExit(s, exit).validators[i].exitEpoch == s.validators[i].exitEpoch
-    //     ensures forall i :: 0 <= i < |s.validators| && i != exit.validator_index as int ==> updateVoluntaryExit(s, exit).validators[i].slashed == s.validators[i].slashed
-    //     ensures forall i :: 0 <= i < |s.validators| && i != exit.validator_index as int ==> updateVoluntaryExit(s, exit).validators[i].withdrawable_epoch == s.validators[i].withdrawable_epoch
-    // {
-    //     // Thanks Dafny
-    // }
-
+    
     lemma mappingVolExitIndices(ve: seq<VoluntaryExit>)
         ensures forall i :: 0 <= i < |ve| ==> get_VolExit_validator_indices(ve)[i] == ve[i].validator_index as int
     {
@@ -468,16 +269,6 @@ module ProcessOperationsProofs {
             assert forall j :: 0 <= j < |ve| ==> get_VolExit_validator_indices(ve)[j] == ve[j].validator_index as int;
         }
     }
-
-    // //lemma PSpreconditionLemma()
-    // lemma helperVolExitLemma4(ve : seq<VoluntaryExit>)
-    //     requires |ve| > 0
-    //     requires forall i,j :: 0 <= i < j < |ve| && i != j ==> ve[i].validator_index!= ve[j].validator_index // ve indices are unique
-    //     ensures ve[|ve|-1].validator_index as int !in get_VolExit_validator_indices(ve[..|ve|-1])
-    // {
-    //     mappingVolExitIndices(ve[..|ve|-1]);
-    //     assert forall i :: 0 <= i < |ve[..|ve|-1]| ==> get_VolExit_validator_indices(ve[..|ve|-1])[i] == ve[i].validator_index as int;
-    // }
 
     
 
